IMLTT/untyped/Weakening.lean
@@ -57,7 +57,7 @@ def weaken (ρ : Weak m n) (t : Tm n) : Tm m :=
   | .refl A a => .refl (weaken ρ A) (weaken ρ a)
   | .firstSigma p => .firstSigma (weaken ρ p)
   | .secondSigma p => .secondSigma (weaken ρ p)
-  | .j A B b a a' p => .j (weaken ρ A) (weaken (lift_weak_n 3 ρ) B) (weaken ρ b)
+  | .j A B b a a' p => .j (weaken ρ A) (weaken (lift_weak_n 3 ρ) B) (weaken (lift_weak_n 1 ρ) b)
                         (weaken ρ a) (weaken ρ a') (weaken ρ p)
 
 def shift_tm : Tm n → Tm (n + 1)
