IMLTT/typed/PropositionalEquality.lean
@@ -1,0 +1,30 @@
+import IMLTT.untyped.AbstractSyntax
+import IMLTT.untyped.Weakening
+import IMLTT.untyped.Substitution
+
+import IMLTT.typed.JudgmentsAndRules
+import IMLTT.typed.proofs.admissable.Weakening
+import IMLTT.typed.proofs.admissable.Substitution
+import IMLTT.typed.proofs.admissable.WeakSubstitution.WeakSubstitution
+import IMLTT.typed.proofs.admissable.Inversion
+import IMLTT.typed.proofs.admissable.FunctionalityTyping
+import IMLTT.typed.proofs.admissable.ContextConv
+
+-- identity of indiscernibles - leibniz principle:
+-- ΠA;(ΠA;(v(1) ≃[A⌊↑ₚ↑ₚidₚ⌋] v(0)) ≃ (Π(ΠA;B); (x ∶ P(A)) ≃ (y ∶ P(A))))
+
+-- ((ΠP; P⌊↑ₚidₚ⌋)⌊↑ₚ↑ₚidₚ⌋) -> Π P(v(1)); P(v(0))
+theorem leibniz_priniple {n : Nat} {Γ : Ctx n} {A p a a' h : Tm n} {B : Tm (n + 3)} {h' P : Tm (n + 1)} :
+    -- Γ ⊢ A type
+    -- → (Γ ⊢ a ∶ A)
+    -- → (Γ ⊢ a' ∶ A)
+    (Γ ⊢ p ∶ a ≃[A] a')
+    → (Γ ⬝ A ⊢ P type)
+    → (Γ ⊢ h ∶ P⌈a⌉₀)
+    → (Γ ⬝ A ⬝ A⌊↑ₚidₚ⌋ ⬝ v(1) ≃[A⌊↑ₚ↑ₚidₚ⌋] v(0)) ⊢ P⌊↑ₚ↑ₚidₚ⌋ type
+    → (Γ ⊢ (.j A ((ΠP; P⌊↑ₚidₚ⌋)⌊↑ₚ↑ₚidₚ⌋) (λ(P); v(0)) a a' p) ◃ h ∶ P⌈a'⌉₀)
+    :=
+  by
+    intro hpId hP hhP _
+    apply HasType.pi_elim (Γ := Γ) (f := (.j A ((ΠP; P⌊↑ₚidₚ⌋)⌊↑ₚ↑ₚidₚ⌋) (λ(P); v(0)) a a' p)) (a := h)
+    sorry
