IMLTT/typed/proofs/admissable/Substitution/HasType.lean
@@ -843,24 +843,22 @@ theorem substitution_gen_nat_elim :
       · rfl
 
 theorem substitution_gen_iden_elim : 
-    ∀ {n : Nat} {Γ : Ctx n} {A : Tm n} {B : Tm (n + 1 + 1 + 1)} {b a a' p : Tm n},
-    (Γ ⬝ A ⬝ A⌊↑ₚidₚ⌋ ⬝ v(1) ≃[A⌊↑ₚ↑ₚidₚ⌋] v(0)) ⊢ B type →
-    (Γ ⊢ b ∶ B⌈(ₛidₚ), a, a, A.refl a⌉) →
+    ∀ {n : Nat} {Γ : Ctx n} {A : Tm n} {B : Tm (n + 1 + 1 + 1)} {b : Tm (n + 1)} {a a' p : Tm n},
+  (Γ ⬝ A ⬝ A⌊↑ₚidₚ⌋ ⬝ v(1) ≃[A⌊↑ₚ↑ₚidₚ⌋] v(0)) ⊢ B type →
+    (Γ ⬝ A ⊢ b ∶ B⌈(ₛidₚ), v(0), (A⌊↑ₚidₚ⌋.refl v(0))⌉) →
       (Γ ⊢ a ∶ A) →
         (Γ ⊢ a' ∶ A) →
           (Γ ⊢ p ∶ a ≃[A] a') →
-            Γ ⊢ B⌈(ₛidₚ), a, a, A.refl a⌉ type →
-              Γ ⊢ B⌈(ₛidₚ), a, a', p⌉ type →
                 (∀ (m l : Nat) {leq : l ≤ m} (Γ_1 : Ctx l) (Δ : CtxGen (l + 1) (m + 1)) (eqM : n + 1 + 1 + 1 = m + 1)
                     {s S : Tm l} (A_1 : Tm (m + 1 - 1 + 1)),
                     (eqM ▸ Γ ⬝ A ⬝ A⌊↑ₚidₚ⌋ ⬝ v(1) ≃[A⌊↑ₚ↑ₚidₚ⌋] v(0)) = Γ_1 ⬝ S ⊗ Δ →
                       eqM ▸ B = A_1 → (Γ_1 ⊢ s ∶ S) → Γ_1 ⊗ ⌈s⌉(Δ w/Nat.le_refl l) ⊢ A_1⌈s/ₙleq⌉ type) →
-                  (∀ (m l : Nat) {leq : l ≤ m} (Γ_1 : Ctx l) (Δ : CtxGen (l + 1) (m + 1)) (eqM : n = m + 1) (s S : Tm l)
-                      (a_7 A_1 : Tm (m + 1 - 1 + 1)),
-                      eqM ▸ Γ = Γ_1 ⬝ S ⊗ Δ →
-                        eqM ▸ b = a_7 →
-                          eqM ▸ B⌈(ₛidₚ), a, a, A.refl a⌉ = A_1 →
-                            (Γ_1 ⊢ s ∶ S) → Γ_1 ⊗ ⌈s⌉(Δ w/Nat.le_refl l) ⊢ a_7⌈s/ₙleq⌉ ∶ A_1⌈s/ₙleq⌉) →
+                  (∀ (m l : Nat) {leq : l ≤ m} (Γ_1 : Ctx l) (Δ : CtxGen (l + 1) (m + 1)) (eqM : n + 1 = m + 1)
+                      (s S : Tm l) (a A_1 : Tm (m + 1 - 1 + 1)),
+                      eqM ▸ Γ ⬝ A = Γ_1 ⬝ S ⊗ Δ →
+                        eqM ▸ b = a →
+                          eqM ▸ B⌈(ₛidₚ), v(0), (A⌊↑ₚidₚ⌋.refl v(0))⌉ = A_1 →
+                            (Γ_1 ⊢ s ∶ S) → Γ_1 ⊗ ⌈s⌉(Δ w/Nat.le_refl l) ⊢ a⌈s/ₙleq⌉ ∶ A_1⌈s/ₙleq⌉) →
                     (∀ (m l : Nat) {leq : l ≤ m} (Γ_1 : Ctx l) (Δ : CtxGen (l + 1) (m + 1)) (eqM : n = m + 1)
                         (s S : Tm l) (a_8 A_1 : Tm (m + 1 - 1 + 1)),
                         eqM ▸ Γ = Γ_1 ⬝ S ⊗ Δ →
@@ -877,16 +875,6 @@ theorem substitution_gen_iden_elim :
                               eqM ▸ p = a_10 →
                                 (eqM ▸ a ≃[A] a') = A_1 →
                                   (Γ_1 ⊢ s ∶ S) → Γ_1 ⊗ ⌈s⌉(Δ w/Nat.le_refl l) ⊢ a_10⌈s/ₙleq⌉ ∶ A_1⌈s/ₙleq⌉) →
-                          (∀ (m l : Nat) {leq : l ≤ m} (Γ_1 : Ctx l) (Δ : CtxGen (l + 1) (m + 1)) (eqM : n = m + 1)
-                              {s S : Tm l} (A_1 : Tm (m + 1 - 1 + 1)),
-                              eqM ▸ Γ = Γ_1 ⬝ S ⊗ Δ →
-                                eqM ▸ B⌈(ₛidₚ), a, a, A.refl a⌉ = A_1 →
-                                  (Γ_1 ⊢ s ∶ S) → Γ_1 ⊗ ⌈s⌉(Δ w/Nat.le_refl l) ⊢ A_1⌈s/ₙleq⌉ type) →
-                            (∀ (m l : Nat) {leq : l ≤ m} (Γ_1 : Ctx l) (Δ : CtxGen (l + 1) (m + 1)) (eqM : n = m + 1)
-                                {s S : Tm l} (A : Tm (m + 1 - 1 + 1)),
-                                eqM ▸ Γ = Γ_1 ⬝ S ⊗ Δ →
-                                  eqM ▸ B⌈(ₛidₚ), a, a', p⌉ = A →
-                                    (Γ_1 ⊢ s ∶ S) → Γ_1 ⊗ ⌈s⌉(Δ w/Nat.le_refl l) ⊢ A⌈s/ₙleq⌉ type) →
                               ∀ (m l : Nat) {leq : l ≤ m} (Γ_1 : Ctx l) (Δ : CtxGen (l + 1) (m + 1)) (eqM : n = m + 1)
                                 (s S : Tm l) (a_13 A_1 : Tm (m + 1 - 1 + 1)),
                                 eqM ▸ Γ = Γ_1 ⬝ S ⊗ Δ →
@@ -894,7 +882,7 @@ theorem substitution_gen_iden_elim :
                                     eqM ▸ B⌈(ₛidₚ), a, a', p⌉ = A_1 →
                                       (Γ_1 ⊢ s ∶ S) → Γ_1 ⊗ ⌈s⌉(Δ w/Nat.le_refl l) ⊢ a_13⌈s/ₙleq⌉ ∶ A_1⌈s/ₙleq⌉ :=
   by
-    intro n Γ' A B b a a' p hB hbB haA haA' hpId hBa hBc ihB ihbB ihaA ihaA' ihpId ihBa ihBc m l hleq Γ Δ heqM s S t T heqΓ heqt heqT hsS
+    intro n Γ' A B b a a' p hB hbB haA haA' hpId ihB ihbB ihaA ihaA' ihpId m l hleq Γ Δ heqM s S t T heqΓ heqt heqT hsS
     cases heqM
     cases heqΓ
     cases heqt
@@ -920,8 +908,11 @@ theorem substitution_gen_iden_elim :
       · rfl
       · apply hsS
       · rfl
-    · rw [←substitution_refl]
-      rw [←subst_subst_iden_elim]
+    · rw [←substitution_shift_id_lift]
+      rw [subst_subst_iden_refl]
+      rw [extend_expand_context_n_substitution]
+      simp [lift_subst_n]
+      rw [lift_n_substitution]
       apply ihbB
       · rfl
       · rfl
@@ -943,19 +934,6 @@ theorem substitution_gen_iden_elim :
     · rw [←substitution_iden]
       apply ihpId
       · rfl
-      · rfl
-      · rfl
-      · apply hsS
-      · rfl
-    · rw [←substitution_refl]
-      rw [←subst_subst_iden_elim]
-      apply ihBa
-      · rfl
-      · rfl
-      · apply hsS
-      · rfl
-    · rw [←subst_subst_iden_elim]
-      apply ihBc
       · rfl
       · rfl
       · apply hsS
