IMLTT/typed/proofs/boundary/IsEqualTerm.lean
@@ -13,207 +13,205 @@ import IMLTT.typed.proofs.admissable.ContextConv
 import IMLTT.typed.proofs.boundary.BoundaryIsCtx
 import IMLTT.typed.proofs.boundary.Helpers
 
-theorem boundary_var_eq :
-    ∀ {x : Nat} {Γ : Ctx x} {A : Tm x},
-    Γ ⊢ A type → Γ ⊢ A type → (Γ ⬝ A ⊢ v(0) ∶ A⌊↑ₚidₚ⌋) ∧ (Γ ⬝ A ⊢ v(0) ∶ A⌊↑ₚidₚ⌋) ∧ Γ ⬝ A ⊢ A⌊↑ₚidₚ⌋ type :=
-  by
-    intro n Γ A hA ihA
-    apply And.intro
-    · apply HasType.var hA
-    · apply And.intro
-      · apply HasType.var hA
-      · apply weakening_type hA hA
-
-theorem boundary_weak_eq :
-    ∀ {x : Nat} {i : Fin x} {Γ : Ctx x} {A B : Tm x},
-    (Γ ⊢ v(i) ≡ v(i) ∶ A) →
-    Γ ⊢ B type →
-    (Γ ⊢ v(i) ∶ A) ∧ (Γ ⊢ v(i) ∶ A) ∧ Γ ⊢ A type →
-    Γ ⊢ B type → (Γ ⬝ B ⊢ v(i)⌊↑ₚidₚ⌋ ∶ A⌊↑ₚidₚ⌋) ∧ (Γ ⬝ B ⊢ v(i)⌊↑ₚidₚ⌋ ∶ A⌊↑ₚidₚ⌋) ∧ Γ ⬝ B ⊢ A⌊↑ₚidₚ⌋ type :=
-  by
-    intro n x Γ A B hvvA hB ihvvA ihB
-    apply And.intro
-    · apply HasType.weak
-      · apply And.left ihvvA
-      · apply ihB
-    · apply And.intro
-      · apply HasType.weak
-        · apply And.left ihvvA
-        · apply ihB
-      · apply weakening_type
-        · apply And.right (And.right ihvvA)
-        · apply ihB
-
-theorem boundary_unit_comp :
-    ∀ {n : Nat} {Γ : Ctx n} {A : Tm (n + 1)} {a : Tm n},
-    Γ ⬝ 𝟙 ⊢ A type →
-    (Γ ⊢ a ∶ A⌈⋆⌉₀) → Γ ⬝ 𝟙 ⊢ A type → Γ ⊢ A⌈⋆⌉₀ type → (Γ ⊢ A.indUnit ⋆ a ∶ A⌈⋆⌉₀) ∧ (Γ ⊢ a ∶ A⌈⋆⌉₀) ∧ Γ ⊢ A⌈⋆⌉₀ type :=
-  by
-    intro n Γ A a hA haA ihA ihaA
-    repeat' apply And.intro
-    · apply HasType.unit_elim
-      · apply hA
-      · apply haA
-      · apply HasType.unit_intro
-        apply boundary_ctx_term haA
-    · apply haA
-    · apply ihaA
-
-theorem boundary_pi_comp :
-    ∀ {n : Nat} {Γ : Ctx n} {A : Tm n} {b B : Tm (n + 1)} {a : Tm n},
-    (Γ ⬝ A ⊢ b ∶ B) →
-    (Γ ⊢ a ∶ A) → Γ ⬝ A ⊢ B type → Γ ⊢ A type → (Γ ⊢ (λA; b)◃a ∶ B⌈a⌉₀) ∧ (Γ ⊢ b⌈a⌉₀ ∶ B⌈a⌉₀) ∧ Γ ⊢ B⌈a⌉₀ type :=
-  by
-    intro n Γ A b B a hbB haA ihbB ihaA
-    repeat' apply And.intro
-    · apply HasType.pi_elim
-      · apply HasType.pi_intro
-        apply hbB
-      · apply haA
-    · apply substitution_term
-      · apply haA
-      · apply hbB
-    · apply substitution_type
-      · apply haA
-      · apply ihbB
-
-theorem boundary_sigma_first_comp :
-    ∀ {n : Nat} {Γ : Ctx n} {a b A : Tm n} {B : Tm (n + 1)},
-  (Γ ⊢ a ∶ A) →
-    (Γ ⊢ b ∶ B⌈a⌉₀) →
-      Γ ⊢ ΣA;B type → Γ ⊢ A type → Γ ⊢ B⌈a⌉₀ type → Γ ⊢ ΣA;B type → (Γ ⊢ π₁ a&b ∶ A) ∧ (Γ ⊢ a ∶ A) ∧ Γ ⊢ A type :=
-  by
-    intro n Γ a b A B haA hbB hSi ihaA ihbB ihSi
-    repeat' apply And.intro
-    · apply HasType.sigma_first
-      apply HasType.sigma_intro
-      · apply haA
-      · apply hbB
-      · have h := sigma_is_type_inversion hSi
-        apply And.right h
-    · apply haA
-    · apply ihaA
-
-theorem boundary_sigma_second_comp :
-    ∀ {n : Nat} {Γ : Ctx n} {a b A : Tm n} {B : Tm (n + 1)},
-  (Γ ⊢ a ∶ A) →
-    (Γ ⊢ b ∶ B⌈a⌉₀) →
-      Γ ⊢ ΣA;B type →
-        Γ ⊢ A type →
-          Γ ⊢ B⌈a⌉₀ type → Γ ⊢ ΣA;B type → (Γ ⊢ π₂ a&b ∶ B⌈π₁ a&b⌉₀) ∧ (Γ ⊢ b ∶ B⌈π₁ a&b⌉₀) ∧ Γ ⊢ B⌈π₁ a&b⌉₀ type :=
-  by
-    intro n Γ a b A B haA hbB hSi ihaA ihbB ihSi
-    repeat' apply And.intro
-    · apply HasType.sigma_second
-      apply HasType.sigma_intro
-      · apply haA
-      · apply hbB
-      · have h := sigma_is_type_inversion hSi
-        apply And.right h
-    · apply HasType.ty_conv
-      · apply hbB
-      · have h := sigma_is_type_inversion hSi
-        apply functionality_typing_type
-        · apply And.right h
-        · apply IsEqualTerm.term_symm
-          apply IsEqualTerm.sigma_first_comp
-          · apply haA
-          · apply hbB
-          · apply hSi
-        · apply haA
-        · apply HasType.sigma_first
-          apply HasType.sigma_intro
-          · apply haA
-          · apply hbB
-          · apply And.right h
-    · have h := sigma_is_type_inversion hSi
-      apply substitution_type
-      · apply HasType.sigma_first
-        apply HasType.sigma_intro
-        · apply haA
-        · apply hbB
-        · apply And.right h
-      · apply And.right h
-
-theorem boundary_nat_zero_comp :
-    ∀ {n : Nat} {Γ : Ctx n} {z : Tm n} {A : Tm (n + 1)} {s : Tm (n + 2)},
-    Γ ⬝ 𝒩 ⊢ A type →
-    (Γ ⊢ z ∶ A⌈𝓏⌉₀) →
-      (Γ ⬝ 𝒩 ⬝ A ⊢ s ∶ A⌈(ₛ↑ₚidₚ), 𝓈(v(0))⌉⌊↑ₚidₚ⌋) →
-        (Γ ⊢ 𝓏 ∶ 𝒩) →
-          Γ ⬝ 𝒩 ⊢ A type →
-            Γ ⊢ A⌈𝓏⌉₀ type →
-              Γ ⬝ 𝒩 ⬝ A ⊢ A⌈(ₛ↑ₚidₚ), 𝓈(v(0))⌉⌊↑ₚidₚ⌋ type →
-                Γ ⊢ 𝒩 type → (Γ ⊢ A.indNat z s 𝓏 ∶ A⌈𝓏⌉₀) ∧ (Γ ⊢ z ∶ A⌈𝓏⌉₀) ∧ Γ ⊢ A⌈𝓏⌉₀ type :=
-  by
-    intro n Γ z A s hA hzA hsA hzNat ihA ihzA ihsA ihzNat
-    repeat' apply And.intro
-    · apply HasType.nat_elim
-      · apply hA
-      · apply hzA
-      · apply hsA
-      · apply hzNat
-    · apply hzA
-    · apply substitution_type
-      · apply hzNat
-      · apply hA
-
-theorem boundary_nat_succ_comp :
-    ∀ {n : Nat} {Γ : Ctx n} {z x : Tm n} {A : Tm (n + 1)} {s : Tm (n + 2)},
-    Γ ⬝ 𝒩 ⊢ A type →
-    (Γ ⊢ z ∶ A⌈𝓏⌉₀) →
-      (Γ ⬝ 𝒩 ⬝ A ⊢ s ∶ A⌈(ₛ↑ₚidₚ), 𝓈(v(0))⌉⌊↑ₚidₚ⌋) →
-        (Γ ⊢ x ∶ 𝒩) →
-          Γ ⬝ 𝒩 ⊢ A type →
-            Γ ⊢ A⌈𝓏⌉₀ type →
-              Γ ⬝ 𝒩 ⬝ A ⊢ A⌈(ₛ↑ₚidₚ), 𝓈(v(0))⌉⌊↑ₚidₚ⌋ type →
-                Γ ⊢ 𝒩 type →
-                  (Γ ⊢ A.indNat z s 𝓈(x) ∶ A⌈𝓈(x)⌉₀) ∧ (Γ ⊢ s⌈(ₛidₚ), x, A.indNat z s x⌉ ∶ A⌈𝓈(x)⌉₀) ∧ Γ ⊢ A⌈𝓈(x)⌉₀ type :=
-  by
-    intro n Γ z x A s hA hzA hsA hsNat ihA ihzA ihsA ihsNat
-    repeat' apply And.intro
-    · apply HasType.nat_elim
-      · apply hA
-      · apply hzA
-      · apply hsA
-      · apply HasType.nat_succ_intro hsNat
-    · rw [substitution_separate]
-      rw [←substitution_shift_substitute_zero (A := A⌈𝓈(x)⌉₀)]
-      apply substitution_term
-      · apply HasType.nat_elim
-        · apply hA
-        · apply hzA
-        · apply hsA
-        · apply hsNat
-      · rw [context_to_gen_ctx] at hsA
-        have h := (And.left (And.right (And.right substitution)) (leq := Nat.le_succ n)) hsA hsNat
-        simp [substitute_into_gen_ctx] at h
-        rw [←lift_n_substitution] at h
-        simp [n_substitution_zero] at h
-        simp [zero_substitution] at h
-        simp [←insane] at h
-        simp [substitute_zero]
-        apply h
-        any_goals omega
-    · apply substitution_type
-      · apply HasType.nat_succ_intro hsNat
-      · apply hA
+-- theorem boundary_var_eq :
+--     ∀ {x : Nat} {Γ : Ctx x} {A : Tm x},
+--     Γ ⊢ A type → Γ ⊢ A type → (Γ ⬝ A ⊢ v(0) ∶ A⌊↑ₚidₚ⌋) ∧ (Γ ⬝ A ⊢ v(0) ∶ A⌊↑ₚidₚ⌋) ∧ Γ ⬝ A ⊢ A⌊↑ₚidₚ⌋ type :=
+--   by
+--     intro n Γ A hA ihA
+--     apply And.intro
+--     · apply HasType.var hA
+--     · apply And.intro
+--       · apply HasType.var hA
+--       · apply weakening_type hA hA
+-- 
+-- theorem boundary_weak_eq :
+--     ∀ {x : Nat} {i : Fin x} {Γ : Ctx x} {A B : Tm x},
+--     (Γ ⊢ v(i) ≡ v(i) ∶ A) →
+--     Γ ⊢ B type →
+--     (Γ ⊢ v(i) ∶ A) ∧ (Γ ⊢ v(i) ∶ A) ∧ Γ ⊢ A type →
+--     Γ ⊢ B type → (Γ ⬝ B ⊢ v(i)⌊↑ₚidₚ⌋ ∶ A⌊↑ₚidₚ⌋) ∧ (Γ ⬝ B ⊢ v(i)⌊↑ₚidₚ⌋ ∶ A⌊↑ₚidₚ⌋) ∧ Γ ⬝ B ⊢ A⌊↑ₚidₚ⌋ type :=
+--   by
+--     intro n x Γ A B hvvA hB ihvvA ihB
+--     apply And.intro
+--     · apply HasType.weak
+--       · apply And.left ihvvA
+--       · apply ihB
+--     · apply And.intro
+--       · apply HasType.weak
+--         · apply And.left ihvvA
+--         · apply ihB
+--       · apply weakening_type
+--         · apply And.right (And.right ihvvA)
+--         · apply ihB
+-- 
+-- theorem boundary_unit_comp :
+--     ∀ {n : Nat} {Γ : Ctx n} {A : Tm (n + 1)} {a : Tm n},
+--     Γ ⬝ 𝟙 ⊢ A type →
+--     (Γ ⊢ a ∶ A⌈⋆⌉₀) → Γ ⬝ 𝟙 ⊢ A type → Γ ⊢ A⌈⋆⌉₀ type → (Γ ⊢ A.indUnit ⋆ a ∶ A⌈⋆⌉₀) ∧ (Γ ⊢ a ∶ A⌈⋆⌉₀) ∧ Γ ⊢ A⌈⋆⌉₀ type :=
+--   by
+--     intro n Γ A a hA haA ihA ihaA
+--     repeat' apply And.intro
+--     · apply HasType.unit_elim
+--       · apply hA
+--       · apply haA
+--       · apply HasType.unit_intro
+--         apply boundary_ctx_term haA
+--     · apply haA
+--     · apply ihaA
+-- 
+-- theorem boundary_pi_comp :
+--     ∀ {n : Nat} {Γ : Ctx n} {A : Tm n} {b B : Tm (n + 1)} {a : Tm n},
+--     (Γ ⬝ A ⊢ b ∶ B) →
+--     (Γ ⊢ a ∶ A) → Γ ⬝ A ⊢ B type → Γ ⊢ A type → (Γ ⊢ (λA; b)◃a ∶ B⌈a⌉₀) ∧ (Γ ⊢ b⌈a⌉₀ ∶ B⌈a⌉₀) ∧ Γ ⊢ B⌈a⌉₀ type :=
+--   by
+--     intro n Γ A b B a hbB haA ihbB ihaA
+--     repeat' apply And.intro
+--     · apply HasType.pi_elim
+--       · apply HasType.pi_intro
+--         apply hbB
+--       · apply haA
+--     · apply substitution_term
+--       · apply haA
+--       · apply hbB
+--     · apply substitution_type
+--       · apply haA
+--       · apply ihbB
+-- 
+-- theorem boundary_sigma_first_comp :
+--     ∀ {n : Nat} {Γ : Ctx n} {a b A : Tm n} {B : Tm (n + 1)},
+--   (Γ ⊢ a ∶ A) →
+--     (Γ ⊢ b ∶ B⌈a⌉₀) →
+--       Γ ⊢ ΣA;B type → Γ ⊢ A type → Γ ⊢ B⌈a⌉₀ type → Γ ⊢ ΣA;B type → (Γ ⊢ π₁ a&b ∶ A) ∧ (Γ ⊢ a ∶ A) ∧ Γ ⊢ A type :=
+--   by
+--     intro n Γ a b A B haA hbB hSi ihaA ihbB ihSi
+--     repeat' apply And.intro
+--     · apply HasType.sigma_first
+--       apply HasType.sigma_intro
+--       · apply haA
+--       · apply hbB
+--       · have h := sigma_is_type_inversion hSi
+--         apply And.right h
+--     · apply haA
+--     · apply ihaA
+-- 
+-- theorem boundary_sigma_second_comp :
+--     ∀ {n : Nat} {Γ : Ctx n} {a b A : Tm n} {B : Tm (n + 1)},
+--   (Γ ⊢ a ∶ A) →
+--     (Γ ⊢ b ∶ B⌈a⌉₀) →
+--       Γ ⊢ ΣA;B type →
+--         Γ ⊢ A type →
+--           Γ ⊢ B⌈a⌉₀ type → Γ ⊢ ΣA;B type → (Γ ⊢ π₂ a&b ∶ B⌈π₁ a&b⌉₀) ∧ (Γ ⊢ b ∶ B⌈π₁ a&b⌉₀) ∧ Γ ⊢ B⌈π₁ a&b⌉₀ type :=
+--   by
+--     intro n Γ a b A B haA hbB hSi ihaA ihbB ihSi
+--     repeat' apply And.intro
+--     · apply HasType.sigma_second
+--       apply HasType.sigma_intro
+--       · apply haA
+--       · apply hbB
+--       · have h := sigma_is_type_inversion hSi
+--         apply And.right h
+--     · apply HasType.ty_conv
+--       · apply hbB
+--       · have h := sigma_is_type_inversion hSi
+--         apply functionality_typing_type
+--         · apply And.right h
+--         · apply IsEqualTerm.term_symm
+--           apply IsEqualTerm.sigma_first_comp
+--           · apply haA
+--           · apply hbB
+--           · apply hSi
+--         · apply haA
+--         · apply HasType.sigma_first
+--           apply HasType.sigma_intro
+--           · apply haA
+--           · apply hbB
+--           · apply And.right h
+--     · have h := sigma_is_type_inversion hSi
+--       apply substitution_type
+--       · apply HasType.sigma_first
+--         apply HasType.sigma_intro
+--         · apply haA
+--         · apply hbB
+--         · apply And.right h
+--       · apply And.right h
+-- 
+-- theorem boundary_nat_zero_comp :
+--     ∀ {n : Nat} {Γ : Ctx n} {z : Tm n} {A : Tm (n + 1)} {s : Tm (n + 2)},
+--     Γ ⬝ 𝒩 ⊢ A type →
+--     (Γ ⊢ z ∶ A⌈𝓏⌉₀) →
+--       (Γ ⬝ 𝒩 ⬝ A ⊢ s ∶ A⌈(ₛ↑ₚidₚ), 𝓈(v(0))⌉⌊↑ₚidₚ⌋) →
+--         (Γ ⊢ 𝓏 ∶ 𝒩) →
+--           Γ ⬝ 𝒩 ⊢ A type →
+--             Γ ⊢ A⌈𝓏⌉₀ type →
+--               Γ ⬝ 𝒩 ⬝ A ⊢ A⌈(ₛ↑ₚidₚ), 𝓈(v(0))⌉⌊↑ₚidₚ⌋ type →
+--                 Γ ⊢ 𝒩 type → (Γ ⊢ A.indNat z s 𝓏 ∶ A⌈𝓏⌉₀) ∧ (Γ ⊢ z ∶ A⌈𝓏⌉₀) ∧ Γ ⊢ A⌈𝓏⌉₀ type :=
+--   by
+--     intro n Γ z A s hA hzA hsA hzNat ihA ihzA ihsA ihzNat
+--     repeat' apply And.intro
+--     · apply HasType.nat_elim
+--       · apply hA
+--       · apply hzA
+--       · apply hsA
+--       · apply hzNat
+--     · apply hzA
+--     · apply substitution_type
+--       · apply hzNat
+--       · apply hA
+-- 
+-- theorem boundary_nat_succ_comp :
+--     ∀ {n : Nat} {Γ : Ctx n} {z x : Tm n} {A : Tm (n + 1)} {s : Tm (n + 2)},
+--     Γ ⬝ 𝒩 ⊢ A type →
+--     (Γ ⊢ z ∶ A⌈𝓏⌉₀) →
+--       (Γ ⬝ 𝒩 ⬝ A ⊢ s ∶ A⌈(ₛ↑ₚidₚ), 𝓈(v(0))⌉⌊↑ₚidₚ⌋) →
+--         (Γ ⊢ x ∶ 𝒩) →
+--           Γ ⬝ 𝒩 ⊢ A type →
+--             Γ ⊢ A⌈𝓏⌉₀ type →
+--               Γ ⬝ 𝒩 ⬝ A ⊢ A⌈(ₛ↑ₚidₚ), 𝓈(v(0))⌉⌊↑ₚidₚ⌋ type →
+--                 Γ ⊢ 𝒩 type →
+--                   (Γ ⊢ A.indNat z s 𝓈(x) ∶ A⌈𝓈(x)⌉₀) ∧ (Γ ⊢ s⌈(ₛidₚ), x, A.indNat z s x⌉ ∶ A⌈𝓈(x)⌉₀) ∧ Γ ⊢ A⌈𝓈(x)⌉₀ type :=
+--   by
+--     intro n Γ z x A s hA hzA hsA hsNat ihA ihzA ihsA ihsNat
+--     repeat' apply And.intro
+--     · apply HasType.nat_elim
+--       · apply hA
+--       · apply hzA
+--       · apply hsA
+--       · apply HasType.nat_succ_intro hsNat
+--     · rw [substitution_separate]
+--       rw [←substitution_shift_substitute_zero (A := A⌈𝓈(x)⌉₀)]
+--       apply substitution_term
+--       · apply HasType.nat_elim
+--         · apply hA
+--         · apply hzA
+--         · apply hsA
+--         · apply hsNat
+--       · rw [context_to_gen_ctx] at hsA
+--         have h := (And.left (And.right (And.right substitution)) (leq := Nat.le_succ n)) hsA hsNat
+--         simp [substitute_into_gen_ctx] at h
+--         rw [←lift_n_substitution] at h
+--         simp [n_substitution_zero] at h
+--         simp [zero_substitution] at h
+--         simp [←insane] at h
+--         simp [substitute_zero]
+--         apply h
+--         any_goals omega
+--     · apply substitution_type
+--       · apply HasType.nat_succ_intro hsNat
+--       · apply hA
 
 theorem boundary_iden_comp :
-    ∀ {n : Nat} {Γ : Ctx n} {A : Tm n} {B : Tm (n + 1 + 1 + 1)} {b a : Tm n},
+    ∀ {n : Nat} {Γ : Ctx n} {A : Tm n} {B : Tm (n + 1 + 1 + 1)} {b : Tm (n + 1)} {a : Tm n},
   (Γ ⬝ A ⬝ A⌊↑ₚidₚ⌋ ⬝ v(1) ≃[A⌊↑ₚ↑ₚidₚ⌋] v(0)) ⊢ B type →
-    (Γ ⊢ b ∶ B⌈(ₛidₚ), a, a, A.refl a⌉) →
+    (Γ ⬝ A ⊢ b ∶ B⌈(ₛidₚ), v(0), (A⌊↑ₚidₚ⌋.refl v(0))⌉) →
       (Γ ⊢ a ∶ A) →
-        Γ ⊢ B⌈(ₛidₚ), a, a, A.refl a⌉ type →
-          (Γ ⬝ A ⬝ A⌊↑ₚidₚ⌋ ⬝ v(1) ≃[A⌊↑ₚ↑ₚidₚ⌋] v(0)) ⊢ B type →
-            Γ ⊢ B⌈(ₛidₚ), a, a, A.refl a⌉ type →
-              Γ ⊢ A type →
-                Γ ⊢ B⌈(ₛidₚ), a, a, A.refl a⌉ type →
-                  (Γ ⊢ A.j B b a a (A.refl a) ∶ B⌈(ₛidₚ), a, a, A.refl a⌉) ∧
-                    (Γ ⊢ b ∶ B⌈(ₛidₚ), a, a, A.refl a⌉) ∧ Γ ⊢ B⌈(ₛidₚ), a, a, A.refl a⌉ type
+        (Γ ⬝ A ⬝ A⌊↑ₚidₚ⌋ ⬝ v(1) ≃[A⌊↑ₚ↑ₚidₚ⌋] v(0)) ⊢ B type →
+          Γ ⬝ A ⊢ B⌈(ₛidₚ), v(0), (A⌊↑ₚidₚ⌋.refl v(0))⌉ type →
+            Γ ⊢ A type →
+              (Γ ⊢ A.j B b a a (A.refl a) ∶ B⌈(ₛidₚ), a, a, A.refl a⌉) ∧
+                (Γ ⊢ b⌈a⌉₀ ∶ B⌈(ₛidₚ), a, a, A.refl a⌉) ∧ Γ ⊢ B⌈(ₛidₚ), a, a, A.refl a⌉ type
  :=
   by
-    intro n Γ A B b a hB hbB haA hBa ihB ihbB ihaA ihBa
+    intro n Γ A B b a hB hbB haA ihB ihbB ihaA
     repeat' apply And.intro
     · apply HasType.iden_elim
       · apply hB
@@ -223,239 +221,243 @@ theorem boundary_iden_comp :
       · apply HasType.iden_intro
         · apply ihaA
         · apply haA
-      · apply hBa
-      · apply ihbB
-    · apply hbB
-    · apply ihbB
-
-theorem boundary_unit_intro_eq :
-    ∀ {n : Nat} {Γ : Ctx n}, Γ ctx → Γ ctx → (Γ ⊢ ⋆ ∶ 𝟙) ∧ (Γ ⊢ ⋆ ∶ 𝟙) ∧ Γ ⊢ 𝟙 type :=
-  by
-    intro n Γ hiC ihiC
-    repeat' apply And.intro
-    · apply HasType.unit_intro hiC
-    · apply HasType.unit_intro hiC
-    · apply IsType.unit_form hiC
-
-theorem boundary_unit_elim_eq :
-    ∀ {n : Nat} {Γ : Ctx n} {A A' : Tm (n + 1)} {a a' b b' : Tm n},
-    Γ ⬝ 𝟙 ⊢ A ≡ A' type →
-    (Γ ⊢ a ≡ a' ∶ A⌈⋆⌉₀) →
-    (Γ ⊢ b ≡ b' ∶ 𝟙) →
-    Γ ⬝ 𝟙 ⊢ A type ∧ Γ ⬝ 𝟙 ⊢ A' type →
-    (Γ ⊢ a ∶ A⌈⋆⌉₀) ∧ (Γ ⊢ a' ∶ A⌈⋆⌉₀) ∧ Γ ⊢ A⌈⋆⌉₀ type →
-    (Γ ⊢ b ∶ 𝟙) ∧ (Γ ⊢ b' ∶ 𝟙) ∧ Γ ⊢ 𝟙 type →
-    (Γ ⊢ A.indUnit b a ∶ A⌈b⌉₀) ∧ (Γ ⊢ A'.indUnit b' a' ∶ A⌈b⌉₀) ∧ Γ ⊢ A⌈b⌉₀ type :=
-  by
-    intro n Γ A A' a a' b b' hAA haaA hbb1 ihAA ihaaA ihbb1
-    repeat' apply And.intro
-    · apply HasType.unit_elim
-      · apply And.left ihAA
-      · apply And.left ihaaA
-      · apply And.left ihbb1
-    · apply HasType.ty_conv
-      · apply HasType.unit_elim
-        · apply And.right ihAA
-        · apply HasType.ty_conv
-          · apply And.left (And.right ihaaA)
-          · apply substitution_type_eq
-            · apply HasType.unit_intro (boundary_ctx_term_eq haaA)
-            · apply hAA
-        · apply And.left (And.right ihbb1)
-      · have hAA' := substitution_type_eq (And.left (And.right ihbb1)) (hAA)
-        apply IsEqualType.type_trans
-        · apply IsEqualType.type_symm hAA'
-        · apply functionality_typing_type
-          · apply And.left ihAA
-          · apply IsEqualTerm.term_symm hbb1
-          · apply And.left (And.right ihbb1)
-          · apply And.left ihbb1
-    · apply substitution_type
-      · apply And.left ihbb1
-      · apply And.left ihAA
-
-theorem boundary_empty_elim_eq :
-    ∀ {n : Nat} {Γ : Ctx n} {A A' : Tm (n + 1)} {b b' : Tm n},
-    Γ ⬝ 𝟘 ⊢ A ≡ A' type →
-    (Γ ⊢ b ≡ b' ∶ 𝟘) →
-    Γ ⬝ 𝟘 ⊢ A type ∧ Γ ⬝ 𝟘 ⊢ A' type →
-    (Γ ⊢ b ∶ 𝟘) ∧ (Γ ⊢ b' ∶ 𝟘) ∧ Γ ⊢ 𝟘 type →
-    (Γ ⊢ A.indEmpty b ∶ A⌈b⌉₀) ∧ (Γ ⊢ A'.indEmpty b' ∶ A⌈b⌉₀) ∧ Γ ⊢ A⌈b⌉₀ type :=
-  by
-    intro n Γ A A' b b' hAA hbb0 ihAA ihbb0
-    repeat' apply And.intro
-    · apply HasType.empty_elim
-      · apply And.left ihAA
-      · apply And.left ihbb0
-    · apply HasType.ty_conv
-      · apply HasType.empty_elim
-        · apply And.right ihAA
-        · apply HasType.ty_conv
-          · apply And.left (And.right ihbb0)
-          · apply IsEqualType.empty_form_eq (boundary_ctx_term_eq hbb0)
-      · have hAA' := substitution_type_eq (And.left (And.right ihbb0)) (hAA)
-        apply IsEqualType.type_trans
-        · apply IsEqualType.type_symm hAA'
-        · apply functionality_typing_type
-          · apply And.left ihAA
-          · apply IsEqualTerm.term_symm hbb0
-          · apply And.left (And.right ihbb0)
-          · apply And.left ihbb0
-    · apply substitution_type
-      · apply And.left ihbb0
-      · apply And.left ihAA
-
-theorem boundary_pi_intro_eq :
-    ∀ {n : Nat} {Γ : Ctx n} {A A' : Tm n} {b b' B : Tm (n + 1)},
-    (Γ ⬝ A ⊢ b ≡ b' ∶ B) →
-    Γ ⊢ A ≡ A' type →
-    (Γ ⬝ A ⊢ b ∶ B) ∧ (Γ ⬝ A ⊢ b' ∶ B) ∧ Γ ⬝ A ⊢ B type →
-    Γ ⊢ A type ∧ Γ ⊢ A' type → (Γ ⊢ λA; b ∶ ΠA;B) ∧ (Γ ⊢ λA'; b' ∶ ΠA;B) ∧ Γ ⊢ ΠA;B type :=
-  by
-    intro n Γ A A' b b' B hbbB hAA ihbbB ihAA
-    repeat' apply And.intro
-    · apply HasType.pi_intro
-      apply And.left ihbbB
-    · apply HasType.ty_conv
-      · apply HasType.pi_intro
-        · apply context_conversion_term
-          · apply And.right ihAA
-          · apply hAA
-          · apply And.left (And.right ihbbB)
-      · apply IsEqualType.pi_form_eq
-        · apply IsEqualType.type_symm hAA
-        · apply defeq_refl_type
-          apply context_conversion_type
-          · apply And.right ihAA
-          · apply hAA
-          · apply And.right (And.right ihbbB)
-    · apply IsType.pi_form
-      · apply And.left ihAA
-      · apply And.right (And.right ihbbB)
-
-theorem boundary_pi_elim_eq :
-    ∀ {n : Nat} {Γ : Ctx n} {f f' A : Tm n} {B : Tm (n + 1)} {a a' : Tm n},
-    (Γ ⊢ f ≡ f' ∶ ΠA;B) →
-    (Γ ⊢ a ≡ a' ∶ A) →
-    (Γ ⊢ f ∶ ΠA;B) ∧ (Γ ⊢ f' ∶ ΠA;B) ∧ Γ ⊢ ΠA;B type →
-    (Γ ⊢ a ∶ A) ∧ (Γ ⊢ a' ∶ A) ∧ Γ ⊢ A type → (Γ ⊢ f◃a ∶ B⌈a⌉₀) ∧ (Γ ⊢ f'◃a' ∶ B⌈a⌉₀) ∧ Γ ⊢ B⌈a⌉₀ type :=
-  by
-    intro n Γ f f' A B a a' hffpi haaA ihffPi ihaaA
-    repeat' apply And.intro
-    · apply HasType.pi_elim
-      · apply And.left ihffPi
-      · apply And.left ihaaA
-    · apply HasType.ty_conv
-      · apply HasType.pi_elim
-        · apply And.left (And.right ihffPi)
-        · apply And.left (And.right ihaaA)
-      · have hPiInv := pi_is_type_inversion (And.right (And.right ihffPi))
-        apply functionality_typing_type
-        · apply And.right hPiInv
-        · apply IsEqualTerm.term_symm haaA
-        · apply And.left (And.right ihaaA)
-        · apply And.left (ihaaA)
-    · apply substitution_type
-      · apply And.left ihaaA
-      · have hPiInv := pi_is_type_inversion (And.right (And.right ihffPi))
-        apply And.right hPiInv
-
-theorem boundary_sigma_intro_eq :
-    ∀ {n : Nat} {Γ : Ctx n} {a a' A b b' : Tm n} {B : Tm (n + 1)},
-    (Γ ⊢ a ≡ a' ∶ A) →
-    (Γ ⊢ b ≡ b' ∶ B⌈a⌉₀) →
-      Γ ⬝ A ⊢ B type →
-        (Γ ⊢ a ∶ A) ∧ (Γ ⊢ a' ∶ A) ∧ Γ ⊢ A type →
-          (Γ ⊢ b ∶ B⌈a⌉₀) ∧ (Γ ⊢ b' ∶ B⌈a⌉₀) ∧ Γ ⊢ B⌈a⌉₀ type →
-            Γ ⬝ A ⊢ B type → (Γ ⊢ a&b ∶ ΣA;B) ∧ (Γ ⊢ a'&b' ∶ ΣA;B) ∧ Γ ⊢ ΣA;B type :=
-  by
-    intro n Γ a a' A b b' B haaA hbbB hB ihaaA ihbbB ihB
-    repeat' apply And.intro
-    · apply HasType.sigma_intro
-      · apply And.left ihaaA
-      · apply And.left ihbbB
-      · apply hB
-    · apply HasType.ty_conv
-      · apply HasType.sigma_intro
-        · apply And.left (And.right ihaaA)
-        · apply HasType.ty_conv
-          · apply And.left (And.right ihbbB)
-          · apply functionality_typing_type
-            · apply hB
-            · apply haaA
-            · apply And.left ihaaA
-            · apply And.left (And.right ihaaA)
-        · apply hB
-      · apply defeq_refl_type
-        apply IsType.sigma_form
-        · apply And.right (And.right ihaaA)
-        · apply hB
-    · apply IsType.sigma_form
-      · apply And.right (And.right ihaaA)
-      · apply hB
-
-theorem boundary_sigma_first_eq :
-    ∀ {n : Nat} {Γ : Ctx n} {p p' A : Tm n} {B : Tm (n + 1)},
-    (Γ ⊢ p ≡ p' ∶ ΣA;B) → (Γ ⊢ p ∶ ΣA;B) ∧ (Γ ⊢ p' ∶ ΣA;B) ∧ Γ ⊢ ΣA;B type → (Γ ⊢ π₁ p ∶ A) ∧ (Γ ⊢ π₁ p' ∶ A) ∧ Γ ⊢ A type :=
-  by
-    intro n Γ p p' A B hppSi ihppSi
-    repeat' apply And.intro
-    · apply HasType.sigma_first
-      apply And.left ihppSi
-    · apply HasType.sigma_first
-      apply And.left (And.right ihppSi)
-    · have h := sigma_is_type_inversion (And.right (And.right ihppSi))
-      apply And.left h
-
-theorem boundary_sigma_second_eq :
-    ∀ {n : Nat} {Γ : Ctx n} {p p' A : Tm n} {B : Tm (n + 1)},
-    (Γ ⊢ p ≡ p' ∶ ΣA;B) →
-    (Γ ⊢ p ∶ ΣA;B) ∧ (Γ ⊢ p' ∶ ΣA;B) ∧ Γ ⊢ ΣA;B type →
-      (Γ ⊢ π₂ p ∶ B⌈π₁ p⌉₀) ∧ (Γ ⊢ π₂ p' ∶ B⌈π₁ p⌉₀) ∧ Γ ⊢ B⌈π₁ p⌉₀ type :=
-  by
-    intro n Γ p p' A B hppSi ihppSi
-    repeat' apply And.intro
-    · apply HasType.sigma_second
-      apply And.left ihppSi
-    · apply HasType.ty_conv
-      · apply HasType.sigma_second
-        apply And.left (And.right ihppSi)
-      · have h := sigma_is_type_inversion (And.right (And.right ihppSi))
-        apply functionality_typing_type
-        · apply And.right h
-        · apply IsEqualTerm.term_symm
-          apply IsEqualTerm.sigma_first_eq
-          apply hppSi
-        · apply HasType.sigma_first
-          apply And.left (And.right ihppSi)
-        · apply HasType.sigma_first
-          apply And.left ihppSi
-    · have h := sigma_is_type_inversion (And.right (And.right ihppSi))
+    · rw [←old_test_hahah]
+      apply substitution_term
+      · apply haA
+      · apply hbB
+    · rw [←old_test_hahah]
       apply substitution_type
-      · apply HasType.sigma_first
-        apply And.left ihppSi
-      · apply And.right h
+      · apply haA
+      · apply ihbB
 
-theorem boundary_nat_zero_intro_eq :
-    ∀ {n : Nat} {Γ : Ctx n}, Γ ctx → Γ ctx → (Γ ⊢ 𝓏 ∶ 𝒩) ∧ (Γ ⊢ 𝓏 ∶ 𝒩) ∧ Γ ⊢ 𝒩 type :=
-  by
-    intro n Γ hiC ihiC
-    repeat' apply And.intro
-    · apply HasType.nat_zero_intro hiC
-    · apply HasType.nat_zero_intro hiC
-    · apply IsType.nat_form hiC
-
-theorem boundary_nat_succ_intro_eq :
-    ∀ {n : Nat} {Γ : Ctx n} {x x' : Tm n},
-    (Γ ⊢ x ≡ x' ∶ 𝒩) → (Γ ⊢ x ∶ 𝒩) ∧ (Γ ⊢ x' ∶ 𝒩) ∧ Γ ⊢ 𝒩 type → (Γ ⊢ 𝓈(x) ∶ 𝒩) ∧ (Γ ⊢ 𝓈(x') ∶ 𝒩) ∧ Γ ⊢ 𝒩 type :=
-  by
-    intro n Γ x x' hxxNat ihxxNat
-    repeat' apply And.intro
-    · apply HasType.nat_succ_intro
-      apply And.left ihxxNat
-    · apply HasType.nat_succ_intro
-      apply And.left (And.right ihxxNat)
-    · apply And.right (And.right ihxxNat)
+-- theorem boundary_unit_intro_eq :
+--     ∀ {n : Nat} {Γ : Ctx n}, Γ ctx → Γ ctx → (Γ ⊢ ⋆ ∶ 𝟙) ∧ (Γ ⊢ ⋆ ∶ 𝟙) ∧ Γ ⊢ 𝟙 type :=
+--   by
+--     intro n Γ hiC ihiC
+--     repeat' apply And.intro
+--     · apply HasType.unit_intro hiC
+--     · apply HasType.unit_intro hiC
+--     · apply IsType.unit_form hiC
+-- 
+-- theorem boundary_unit_elim_eq :
+--     ∀ {n : Nat} {Γ : Ctx n} {A A' : Tm (n + 1)} {a a' b b' : Tm n},
+--     Γ ⬝ 𝟙 ⊢ A ≡ A' type →
+--     (Γ ⊢ a ≡ a' ∶ A⌈⋆⌉₀) →
+--     (Γ ⊢ b ≡ b' ∶ 𝟙) →
+--     Γ ⬝ 𝟙 ⊢ A type ∧ Γ ⬝ 𝟙 ⊢ A' type →
+--     (Γ ⊢ a ∶ A⌈⋆⌉₀) ∧ (Γ ⊢ a' ∶ A⌈⋆⌉₀) ∧ Γ ⊢ A⌈⋆⌉₀ type →
+--     (Γ ⊢ b ∶ 𝟙) ∧ (Γ ⊢ b' ∶ 𝟙) ∧ Γ ⊢ 𝟙 type →
+--     (Γ ⊢ A.indUnit b a ∶ A⌈b⌉₀) ∧ (Γ ⊢ A'.indUnit b' a' ∶ A⌈b⌉₀) ∧ Γ ⊢ A⌈b⌉₀ type :=
+--   by
+--     intro n Γ A A' a a' b b' hAA haaA hbb1 ihAA ihaaA ihbb1
+--     repeat' apply And.intro
+--     · apply HasType.unit_elim
+--       · apply And.left ihAA
+--       · apply And.left ihaaA
+--       · apply And.left ihbb1
+--     · apply HasType.ty_conv
+--       · apply HasType.unit_elim
+--         · apply And.right ihAA
+--         · apply HasType.ty_conv
+--           · apply And.left (And.right ihaaA)
+--           · apply substitution_type_eq
+--             · apply HasType.unit_intro (boundary_ctx_term_eq haaA)
+--             · apply hAA
+--         · apply And.left (And.right ihbb1)
+--       · have hAA' := substitution_type_eq (And.left (And.right ihbb1)) (hAA)
+--         apply IsEqualType.type_trans
+--         · apply IsEqualType.type_symm hAA'
+--         · apply functionality_typing_type
+--           · apply And.left ihAA
+--           · apply IsEqualTerm.term_symm hbb1
+--           · apply And.left (And.right ihbb1)
+--           · apply And.left ihbb1
+--     · apply substitution_type
+--       · apply And.left ihbb1
+--       · apply And.left ihAA
+-- 
+-- theorem boundary_empty_elim_eq :
+--     ∀ {n : Nat} {Γ : Ctx n} {A A' : Tm (n + 1)} {b b' : Tm n},
+--     Γ ⬝ 𝟘 ⊢ A ≡ A' type →
+--     (Γ ⊢ b ≡ b' ∶ 𝟘) →
+--     Γ ⬝ 𝟘 ⊢ A type ∧ Γ ⬝ 𝟘 ⊢ A' type →
+--     (Γ ⊢ b ∶ 𝟘) ∧ (Γ ⊢ b' ∶ 𝟘) ∧ Γ ⊢ 𝟘 type →
+--     (Γ ⊢ A.indEmpty b ∶ A⌈b⌉₀) ∧ (Γ ⊢ A'.indEmpty b' ∶ A⌈b⌉₀) ∧ Γ ⊢ A⌈b⌉₀ type :=
+--   by
+--     intro n Γ A A' b b' hAA hbb0 ihAA ihbb0
+--     repeat' apply And.intro
+--     · apply HasType.empty_elim
+--       · apply And.left ihAA
+--       · apply And.left ihbb0
+--     · apply HasType.ty_conv
+--       · apply HasType.empty_elim
+--         · apply And.right ihAA
+--         · apply HasType.ty_conv
+--           · apply And.left (And.right ihbb0)
+--           · apply IsEqualType.empty_form_eq (boundary_ctx_term_eq hbb0)
+--       · have hAA' := substitution_type_eq (And.left (And.right ihbb0)) (hAA)
+--         apply IsEqualType.type_trans
+--         · apply IsEqualType.type_symm hAA'
+--         · apply functionality_typing_type
+--           · apply And.left ihAA
+--           · apply IsEqualTerm.term_symm hbb0
+--           · apply And.left (And.right ihbb0)
+--           · apply And.left ihbb0
+--     · apply substitution_type
+--       · apply And.left ihbb0
+--       · apply And.left ihAA
+-- 
+-- theorem boundary_pi_intro_eq :
+--     ∀ {n : Nat} {Γ : Ctx n} {A A' : Tm n} {b b' B : Tm (n + 1)},
+--     (Γ ⬝ A ⊢ b ≡ b' ∶ B) →
+--     Γ ⊢ A ≡ A' type →
+--     (Γ ⬝ A ⊢ b ∶ B) ∧ (Γ ⬝ A ⊢ b' ∶ B) ∧ Γ ⬝ A ⊢ B type →
+--     Γ ⊢ A type ∧ Γ ⊢ A' type → (Γ ⊢ λA; b ∶ ΠA;B) ∧ (Γ ⊢ λA'; b' ∶ ΠA;B) ∧ Γ ⊢ ΠA;B type :=
+--   by
+--     intro n Γ A A' b b' B hbbB hAA ihbbB ihAA
+--     repeat' apply And.intro
+--     · apply HasType.pi_intro
+--       apply And.left ihbbB
+--     · apply HasType.ty_conv
+--       · apply HasType.pi_intro
+--         · apply context_conversion_term
+--           · apply And.right ihAA
+--           · apply hAA
+--           · apply And.left (And.right ihbbB)
+--       · apply IsEqualType.pi_form_eq
+--         · apply IsEqualType.type_symm hAA
+--         · apply defeq_refl_type
+--           apply context_conversion_type
+--           · apply And.right ihAA
+--           · apply hAA
+--           · apply And.right (And.right ihbbB)
+--     · apply IsType.pi_form
+--       · apply And.left ihAA
+--       · apply And.right (And.right ihbbB)
+-- 
+-- theorem boundary_pi_elim_eq :
+--     ∀ {n : Nat} {Γ : Ctx n} {f f' A : Tm n} {B : Tm (n + 1)} {a a' : Tm n},
+--     (Γ ⊢ f ≡ f' ∶ ΠA;B) →
+--     (Γ ⊢ a ≡ a' ∶ A) →
+--     (Γ ⊢ f ∶ ΠA;B) ∧ (Γ ⊢ f' ∶ ΠA;B) ∧ Γ ⊢ ΠA;B type →
+--     (Γ ⊢ a ∶ A) ∧ (Γ ⊢ a' ∶ A) ∧ Γ ⊢ A type → (Γ ⊢ f◃a ∶ B⌈a⌉₀) ∧ (Γ ⊢ f'◃a' ∶ B⌈a⌉₀) ∧ Γ ⊢ B⌈a⌉₀ type :=
+--   by
+--     intro n Γ f f' A B a a' hffpi haaA ihffPi ihaaA
+--     repeat' apply And.intro
+--     · apply HasType.pi_elim
+--       · apply And.left ihffPi
+--       · apply And.left ihaaA
+--     · apply HasType.ty_conv
+--       · apply HasType.pi_elim
+--         · apply And.left (And.right ihffPi)
+--         · apply And.left (And.right ihaaA)
+--       · have hPiInv := pi_is_type_inversion (And.right (And.right ihffPi))
+--         apply functionality_typing_type
+--         · apply And.right hPiInv
+--         · apply IsEqualTerm.term_symm haaA
+--         · apply And.left (And.right ihaaA)
+--         · apply And.left (ihaaA)
+--     · apply substitution_type
+--       · apply And.left ihaaA
+--       · have hPiInv := pi_is_type_inversion (And.right (And.right ihffPi))
+--         apply And.right hPiInv
+-- 
+-- theorem boundary_sigma_intro_eq :
+--     ∀ {n : Nat} {Γ : Ctx n} {a a' A b b' : Tm n} {B : Tm (n + 1)},
+--     (Γ ⊢ a ≡ a' ∶ A) →
+--     (Γ ⊢ b ≡ b' ∶ B⌈a⌉₀) →
+--       Γ ⬝ A ⊢ B type →
+--         (Γ ⊢ a ∶ A) ∧ (Γ ⊢ a' ∶ A) ∧ Γ ⊢ A type →
+--           (Γ ⊢ b ∶ B⌈a⌉₀) ∧ (Γ ⊢ b' ∶ B⌈a⌉₀) ∧ Γ ⊢ B⌈a⌉₀ type →
+--             Γ ⬝ A ⊢ B type → (Γ ⊢ a&b ∶ ΣA;B) ∧ (Γ ⊢ a'&b' ∶ ΣA;B) ∧ Γ ⊢ ΣA;B type :=
+--   by
+--     intro n Γ a a' A b b' B haaA hbbB hB ihaaA ihbbB ihB
+--     repeat' apply And.intro
+--     · apply HasType.sigma_intro
+--       · apply And.left ihaaA
+--       · apply And.left ihbbB
+--       · apply hB
+--     · apply HasType.ty_conv
+--       · apply HasType.sigma_intro
+--         · apply And.left (And.right ihaaA)
+--         · apply HasType.ty_conv
+--           · apply And.left (And.right ihbbB)
+--           · apply functionality_typing_type
+--             · apply hB
+--             · apply haaA
+--             · apply And.left ihaaA
+--             · apply And.left (And.right ihaaA)
+--         · apply hB
+--       · apply defeq_refl_type
+--         apply IsType.sigma_form
+--         · apply And.right (And.right ihaaA)
+--         · apply hB
+--     · apply IsType.sigma_form
+--       · apply And.right (And.right ihaaA)
+--       · apply hB
+-- 
+-- theorem boundary_sigma_first_eq :
+--     ∀ {n : Nat} {Γ : Ctx n} {p p' A : Tm n} {B : Tm (n + 1)},
+--     (Γ ⊢ p ≡ p' ∶ ΣA;B) → (Γ ⊢ p ∶ ΣA;B) ∧ (Γ ⊢ p' ∶ ΣA;B) ∧ Γ ⊢ ΣA;B type → (Γ ⊢ π₁ p ∶ A) ∧ (Γ ⊢ π₁ p' ∶ A) ∧ Γ ⊢ A type :=
+--   by
+--     intro n Γ p p' A B hppSi ihppSi
+--     repeat' apply And.intro
+--     · apply HasType.sigma_first
+--       apply And.left ihppSi
+--     · apply HasType.sigma_first
+--       apply And.left (And.right ihppSi)
+--     · have h := sigma_is_type_inversion (And.right (And.right ihppSi))
+--       apply And.left h
+-- 
+-- theorem boundary_sigma_second_eq :
+--     ∀ {n : Nat} {Γ : Ctx n} {p p' A : Tm n} {B : Tm (n + 1)},
+--     (Γ ⊢ p ≡ p' ∶ ΣA;B) →
+--     (Γ ⊢ p ∶ ΣA;B) ∧ (Γ ⊢ p' ∶ ΣA;B) ∧ Γ ⊢ ΣA;B type →
+--       (Γ ⊢ π₂ p ∶ B⌈π₁ p⌉₀) ∧ (Γ ⊢ π₂ p' ∶ B⌈π₁ p⌉₀) ∧ Γ ⊢ B⌈π₁ p⌉₀ type :=
+--   by
+--     intro n Γ p p' A B hppSi ihppSi
+--     repeat' apply And.intro
+--     · apply HasType.sigma_second
+--       apply And.left ihppSi
+--     · apply HasType.ty_conv
+--       · apply HasType.sigma_second
+--         apply And.left (And.right ihppSi)
+--       · have h := sigma_is_type_inversion (And.right (And.right ihppSi))
+--         apply functionality_typing_type
+--         · apply And.right h
+--         · apply IsEqualTerm.term_symm
+--           apply IsEqualTerm.sigma_first_eq
+--           apply hppSi
+--         · apply HasType.sigma_first
+--           apply And.left (And.right ihppSi)
+--         · apply HasType.sigma_first
+--           apply And.left ihppSi
+--     · have h := sigma_is_type_inversion (And.right (And.right ihppSi))
+--       apply substitution_type
+--       · apply HasType.sigma_first
+--         apply And.left ihppSi
+--       · apply And.right h
+-- 
+-- theorem boundary_nat_zero_intro_eq :
+--     ∀ {n : Nat} {Γ : Ctx n}, Γ ctx → Γ ctx → (Γ ⊢ 𝓏 ∶ 𝒩) ∧ (Γ ⊢ 𝓏 ∶ 𝒩) ∧ Γ ⊢ 𝒩 type :=
+--   by
+--     intro n Γ hiC ihiC
+--     repeat' apply And.intro
+--     · apply HasType.nat_zero_intro hiC
+--     · apply HasType.nat_zero_intro hiC
+--     · apply IsType.nat_form hiC
+-- 
+-- theorem boundary_nat_succ_intro_eq :
+--     ∀ {n : Nat} {Γ : Ctx n} {x x' : Tm n},
+--     (Γ ⊢ x ≡ x' ∶ 𝒩) → (Γ ⊢ x ∶ 𝒩) ∧ (Γ ⊢ x' ∶ 𝒩) ∧ Γ ⊢ 𝒩 type → (Γ ⊢ 𝓈(x) ∶ 𝒩) ∧ (Γ ⊢ 𝓈(x') ∶ 𝒩) ∧ Γ ⊢ 𝒩 type :=
+--   by
+--     intro n Γ x x' hxxNat ihxxNat
+--     repeat' apply And.intro
+--     · apply HasType.nat_succ_intro
+--       apply And.left ihxxNat
+--     · apply HasType.nat_succ_intro
+--       apply And.left (And.right ihxxNat)
+--     · apply And.right (And.right ihxxNat)
 
 theorem boundary_nat_elim_eq :
     ∀ {n : Nat} {Γ : Ctx n} {z z' x x' : Tm n} {A A' : Tm (n + 1)} {s s' : Tm (n + 2)},
@@ -554,30 +556,27 @@ theorem boundary_iden_intro_eq :
       · apply And.left ihaaA
 
 theorem boundary_iden_elim_eq :
-  ∀ {n : Nat} {Γ : Ctx n} {A : Tm n} {B B' : Tm (n + 1 + 1 + 1)} {b b' a₁ a₃ A' a₂ a₄ p p' : Tm n},
+  ∀ {n : Nat} {Γ : Ctx n} {A : Tm n} {B B' : Tm (n + 1 + 1 + 1)} {b b' : Tm (n + 1)} {a₁ a₃ A' a₂ a₄ p p' : Tm n},
   (Γ ⬝ A ⬝ A⌊↑ₚidₚ⌋ ⬝ v(1) ≃[A⌊↑ₚ↑ₚidₚ⌋] v(0)) ⊢ B ≡ B' type →
-    (Γ ⊢ b ≡ b' ∶ B⌈(ₛidₚ), a₁, a₁, A.refl a₁⌉) →
+    (Γ ⬝ A ⊢ b ≡ b' ∶ B⌈(ₛidₚ), v(0), (A⌊↑ₚidₚ⌋.refl v(0))⌉) →
       Γ ⊢ A ≡ A' type →
         (Γ ⊢ a₁ ≡ a₂ ∶ A) →
           (Γ ⊢ a₃ ≡ a₄ ∶ A') →
             (Γ ⊢ p ≡ p' ∶ a₁ ≃[A] a₃) →
-              Γ ⊢ B⌈(ₛidₚ), a₁, a₁, A.refl a₁⌉ ≡ B'⌈(ₛidₚ), a₂, a₂, A'.refl a₂⌉ type →
-                Γ ⊢ B⌈(ₛidₚ), a₁, a₃, p⌉ ≡ B'⌈(ₛidₚ), a₂, a₄, p'⌉ type →
-                  (Γ ⬝ A ⬝ A⌊↑ₚidₚ⌋ ⬝ v(1) ≃[A⌊↑ₚ↑ₚidₚ⌋] v(0)) ⊢ B type ∧
-                      (Γ ⬝ A ⬝ A⌊↑ₚidₚ⌋ ⬝ v(1) ≃[A⌊↑ₚ↑ₚidₚ⌋] v(0)) ⊢ B' type →
-                    (Γ ⊢ b ∶ B⌈(ₛidₚ), a₁, a₁, A.refl a₁⌉) ∧
-                        (Γ ⊢ b' ∶ B⌈(ₛidₚ), a₁, a₁, A.refl a₁⌉) ∧ Γ ⊢ B⌈(ₛidₚ), a₁, a₁, A.refl a₁⌉ type →
-                      Γ ⊢ A type ∧ Γ ⊢ A' type →
-                        (Γ ⊢ a₁ ∶ A) ∧ (Γ ⊢ a₂ ∶ A) ∧ Γ ⊢ A type →
-                          (Γ ⊢ a₃ ∶ A') ∧ (Γ ⊢ a₄ ∶ A') ∧ Γ ⊢ A' type →
-                            (Γ ⊢ p ∶ a₁ ≃[A] a₃) ∧ (Γ ⊢ p' ∶ a₁ ≃[A] a₃) ∧ Γ ⊢ a₁ ≃[A] a₃ type →
-                              Γ ⊢ B⌈(ₛidₚ), a₁, a₁, A.refl a₁⌉ type ∧ Γ ⊢ B'⌈(ₛidₚ), a₂, a₂, A'.refl a₂⌉ type →
-                                Γ ⊢ B⌈(ₛidₚ), a₁, a₃, p⌉ type ∧ Γ ⊢ B'⌈(ₛidₚ), a₂, a₄, p'⌉ type →
-                                  (Γ ⊢ A.j B b a₁ a₃ p ∶ B⌈(ₛidₚ), a₁, a₃, p⌉) ∧
-                                    (Γ ⊢ A'.j B' b' a₂ a₄ p' ∶ B⌈(ₛidₚ), a₁, a₃, p⌉) ∧ Γ ⊢ B⌈(ₛidₚ), a₁, a₃, p⌉ type
+              (Γ ⬝ A ⬝ A⌊↑ₚidₚ⌋ ⬝ v(1) ≃[A⌊↑ₚ↑ₚidₚ⌋] v(0)) ⊢ B type ∧
+                  (Γ ⬝ A ⬝ A⌊↑ₚidₚ⌋ ⬝ v(1) ≃[A⌊↑ₚ↑ₚidₚ⌋] v(0)) ⊢ B' type →
+                (Γ ⬝ A ⊢ b ∶ B⌈(ₛidₚ), v(0), (A⌊↑ₚidₚ⌋.refl v(0))⌉) ∧
+                    (Γ ⬝ A ⊢ b' ∶ B⌈(ₛidₚ), v(0), (A⌊↑ₚidₚ⌋.refl v(0))⌉) ∧
+                      Γ ⬝ A ⊢ B⌈(ₛidₚ), v(0), (A⌊↑ₚidₚ⌋.refl v(0))⌉ type →
+                  Γ ⊢ A type ∧ Γ ⊢ A' type →
+                    (Γ ⊢ a₁ ∶ A) ∧ (Γ ⊢ a₂ ∶ A) ∧ Γ ⊢ A type →
+                      (Γ ⊢ a₃ ∶ A') ∧ (Γ ⊢ a₄ ∶ A') ∧ Γ ⊢ A' type →
+                        (Γ ⊢ p ∶ a₁ ≃[A] a₃) ∧ (Γ ⊢ p' ∶ a₁ ≃[A] a₃) ∧ Γ ⊢ a₁ ≃[A] a₃ type →
+                          (Γ ⊢ A.j B b a₁ a₃ p ∶ B⌈(ₛidₚ), a₁, a₃, p⌉) ∧
+                            (Γ ⊢ A'.j B' b' a₂ a₄ p' ∶ B⌈(ₛidₚ), a₁, a₃, p⌉) ∧ Γ ⊢ B⌈(ₛidₚ), a₁, a₃, p⌉ type
  :=
   by
-    intro n Γ A B B' b b' a₁ a₃ A' a₂ a₄ p p' hBB hbbB hAA haaA haaA' hppId hBBa hBBc ihBB ihbbB ihAA ihaaA ihaaA' ihppId ihBBa ihBBc
+    intro n Γ A B B' b b' a₁ a₃ A' a₂ a₄ p p' hBB hbbB hAA haaA haaA' hppId ihBB ihbbB ihAA ihaaA ihaaA' ihppId
     repeat' apply And.intro
     · apply HasType.iden_elim
       · apply And.left ihBB
@@ -587,8 +586,6 @@ theorem boundary_iden_elim_eq :
         · apply And.left ihaaA'
         · apply IsEqualType.type_symm hAA
       · apply And.left ihppId
-      · apply And.left ihBBa
-      · apply And.left ihBBc
     · apply HasType.ty_conv
       · apply HasType.iden_elim
         · rw [context_to_gen_ctx]
@@ -685,9 +682,127 @@ theorem boundary_iden_elim_eq :
                       · apply And.left ihAA
                       · apply And.left ihAA
               · apply And.right ihBB
-        · apply HasType.ty_conv
+        · apply context_conversion_term
+          · apply And.right ihAA
+          · apply hAA
+          apply HasType.ty_conv
           · apply And.left (And.right ihbbB)
-          · apply hBBa
+          · rw [context_to_gen_ctx] at hBB
+            have ht :=
+                And.left (And.right (And.right (And.right weak_substitution)))
+                  (leq := Nat.le_step (Nat.le_refl (n + 2)))
+                  hBB
+                  (by
+                    apply HasType.weak
+                    · apply HasType.var (And.left ihAA)
+                    · apply weakening_type (And.left ihAA) (And.left ihAA)
+                  )
+            simp [substitute_shift_into_gen_ctx] at ht
+            simp [n_substitution_shift_zero] at ht
+            simp [vone_to_vtwo] at ht
+            simp [expand_ctx] at ht
+            simp [←lift_n_substitution_shift] at ht
+            have hrefl : Γ ⬝ A ⬝ A⌊↑ₚidₚ⌋ ⊢ (.refl (A⌊↑ₚ↑ₚidₚ⌋) v(1)) ∶ v(1) ≃[A⌊↑ₚ↑ₚidₚ⌋] v(1) :=
+              by apply HasType.iden_intro
+                 · rw (config := {occs := .pos [2]}) [←weakening_shift_id]
+                   apply weakening_type
+                   · apply weakening_type (And.left ihAA) (And.left ihAA)
+                   · apply weakening_type (And.left ihAA) (And.left ihAA)
+                 · rw (config := {occs := .pos [2]}) [←weakening_shift_id]
+                   rw [weakening_shift_vone]
+                   apply HasType.weak
+                   · apply HasType.var (And.left ihAA)
+                   · apply weakening_type (And.left ihAA) (And.left ihAA)
+            apply IsEqualType.type_trans
+            · have hnow := substitution_type_eq hrefl ht
+              simp [weaken] at hnow
+              simp [weaken_var] at hnow
+              have hlol := substitution_type_eq (HasType.var (And.left ihAA)) hnow
+              simp [even_new_test] at hlol
+              apply hlol
+            · rw [context_to_gen_ctx] at ihBB
+              have ht :=
+                  And.left (And.right (weak_substitution))
+                    (leq := Nat.le_step (Nat.le_refl (n + 2)))
+                    (And.right ihBB)
+                    (by
+                      apply HasType.weak
+                      · apply HasType.var (And.left ihAA)
+                      · apply weakening_type (And.left ihAA) (And.left ihAA)
+                    )
+              simp [substitute_shift_into_gen_ctx] at ht
+              simp [n_substitution_shift_zero] at ht
+              simp [vone_to_vtwo] at ht
+              simp [expand_ctx] at ht
+              simp [←lift_n_substitution_shift] at ht
+              have hrefl : Γ ⬝ A ⬝ A⌊↑ₚidₚ⌋ ⊢ (.refl (A⌊↑ₚ↑ₚidₚ⌋) v(1)) ∶ v(1) ≃[A⌊↑ₚ↑ₚidₚ⌋] v(1) :=
+                by apply HasType.iden_intro
+                   · rw (config := {occs := .pos [2]}) [←weakening_shift_id]
+                     apply weakening_type
+                     · apply weakening_type (And.left ihAA) (And.left ihAA)
+                     · apply weakening_type (And.left ihAA) (And.left ihAA)
+                   · rw (config := {occs := .pos [2]}) [←weakening_shift_id]
+                     rw [weakening_shift_vone]
+                     apply HasType.weak
+                     · apply HasType.var (And.left ihAA)
+                     · apply weakening_type (And.left ihAA) (And.left ihAA)
+              have hrefl' : Γ ⬝ A ⬝ A⌊↑ₚidₚ⌋ ⊢ (.refl (A'⌊↑ₚ↑ₚidₚ⌋) v(1)) ∶ v(1) ≃[A⌊↑ₚ↑ₚidₚ⌋] v(1) :=
+                by
+                  apply HasType.ty_conv
+                  · apply HasType.iden_intro
+                    · rw (config := {occs := .pos [2]}) [←weakening_shift_id]
+                      apply weakening_type
+                      · apply weakening_type (And.right ihAA) (And.left ihAA)
+                      · apply weakening_type (And.left ihAA) (And.left ihAA)
+                    · rw (config := {occs := .pos [2]}) [←weakening_shift_id]
+                      rw [weakening_shift_vone]
+                      apply HasType.weak
+                      · apply HasType.ty_conv
+                        · apply HasType.var (And.left ihAA)
+                        · apply weakening_type_eq
+                          · apply hAA
+                          · apply And.left ihAA
+                      · apply weakening_type (And.left ihAA) (And.left ihAA)
+                  · apply IsEqualType.iden_form_eq
+                    rw (config := {occs := .pos [2]}) [←weakening_shift_id]
+                    rw (config := {occs := .pos [4]}) [←weakening_shift_id]
+                    · apply weakening_type_eq
+                      · apply weakening_type_eq
+                        · apply IsEqualType.type_symm hAA
+                        · apply And.left ihAA
+                      · apply weakening_type (And.left ihAA) (And.left ihAA)
+                    · simp [weakening_shift_vone]
+                      rw (config := {occs := .pos [4]}) [←weakening_shift_id]
+                      apply IsEqualTerm.weak_eq
+                      · apply IsEqualTerm.ty_conv_eq
+                        · apply IsEqualTerm.var_eq (And.left ihAA)
+                        · apply weakening_type_eq
+                          · apply hAA
+                          · apply And.left ihAA
+                      · apply weakening_type (And.left ihAA) (And.left ihAA)
+                    · simp [weakening_shift_vone]
+                      rw (config := {occs := .pos [4]}) [←weakening_shift_id]
+                      apply IsEqualTerm.weak_eq
+                      · apply IsEqualTerm.var_eq (And.left ihAA)
+                      · apply weakening_type (And.left ihAA) (And.left ihAA)
+              have hrefleq : Γ ⬝ A ⬝ A⌊↑ₚidₚ⌋ ⊢ (.refl (A⌊↑ₚ↑ₚidₚ⌋) v(1)) ≡ (.refl (A'⌊↑ₚ↑ₚidₚ⌋) v(1)) ∶ v(1) ≃[A⌊↑ₚ↑ₚidₚ⌋] v(1) :=
+                by apply IsEqualTerm.iden_intro_eq
+                   · rw (config := {occs := .pos [2]}) [←weakening_shift_id]
+                     rw (config := {occs := .pos [4]}) [←weakening_shift_id]
+                     apply weakening_type_eq
+                     · apply weakening_type_eq hAA (And.left ihAA)
+                     · apply weakening_type (And.left ihAA) (And.left ihAA)
+                   · rw (config := {occs := .pos [2]}) [←weakening_shift_id]
+                     rw [weakening_shift_vone]
+                     apply IsEqualTerm.weak_eq
+                     · apply IsEqualTerm.var_eq (And.left ihAA)
+                     · apply weakening_type (And.left ihAA) (And.left ihAA)
+              have hnow := functionality_typing_type ht hrefleq hrefl hrefl'
+              simp [weaken] at hnow
+              simp [weaken_var] at hnow
+              have hlol := substitution_type_eq (HasType.var (And.left ihAA)) hnow
+              simp [even_new_test] at hlol
+              apply hlol
         · apply HasType.ty_conv
           · apply And.left (And.right ihaaA)
           · apply hAA
@@ -698,131 +813,293 @@ theorem boundary_iden_elim_eq :
             · apply hAA
             · apply haaA
             · apply haaA'
-        · apply And.right ihBBa
-        · apply And.right ihBBc
       · apply IsEqualType.type_symm
-        apply hBBc
-    · apply And.left ihBBc
+        apply IsEqualType.type_trans
+        rotate_right
+        · apply B'⌈(ₛidₚ), a₁, a₃, p⌉
+        · rw [context_to_gen_ctx] at hBB
+          rw [←middle_expand_context (Γ := Γ ⬝ A)] at hBB
+          have h := And.left (And.right (And.right (And.right substitution))) (leq := Nat.le_step (Nat.le_step (Nat.le_refl n))) hBB (And.left ihaaA)
+          simp [substitute_into_gen_ctx] at h
+          rw [n_substitution_zero] at h
+          rw [zero_substitution] at h
+          rw [substitution_conv_zero] at h
+          rw [substitution_shift_substitute_zero] at h
+          rw [middle_expand_context] at h
+          have h2 := And.left (And.right (And.right (And.right substitution))) (leq := Nat.le_step (Nat.le_refl n)) h (HasType.ty_conv (And.left ihaaA') (IsEqualType.type_symm hAA))
+          simp [substitute_into_gen_ctx] at h2
+          simp [expand_ctx] at h2
+          rw [←lift_n_substitution] at h2
+          simp [n_substitution_zero] at h2
+          simp [zero_substitution] at h2
+          simp [substitution_conv_zero] at h2
+          simp [clean_this_mess_asap] at h2
+          have h3 := substitution_type_eq (And.left ihppId) h2
+          simp [←lift_n_substitution] at h3
+          simp [n_substitution_zero] at h3
+          simp [zero_substitution] at h3
+          simp [clean_this_mess_too] at h3
+          apply h3
+          any_goals omega
+        · apply IsEqualType.type_trans
+          rotate_right
+          · apply B'⌈(ₛidₚ), a₂, a₃, p⌉
+          · rw [context_to_gen_ctx] at ihBB
+            rw [←middle_expand_context (Γ := Γ ⬝ A)] at ihBB
+            have h1 := (And.left (And.right functionality_typing))
+                        haaA (And.left ihaaA) (And.left (And.right ihaaA)) (And.right ihBB)
+            simp [substitute_into_gen_ctx] at h1
+            rw [n_substitution_zero] at h1
+            rw [zero_substitution] at h1
+            rw [substitution_conv_zero] at h1
+            rw [substitution_shift_substitute_zero] at h1
+            rw [middle_expand_context] at h1
+            have h2 := (And.left (And.right (And.right (And.right substitution))) 
+                        (leq := Nat.le_step (Nat.le_refl n)))
+                        h1 (HasType.ty_conv (And.left ihaaA') (IsEqualType.type_symm hAA))
+            simp [substitute_into_gen_ctx] at h2
+            simp [expand_ctx] at h2
+            rw [←lift_n_substitution] at h2
+            simp [n_substitution_zero] at h2
+            simp [zero_substitution] at h2
+            simp [substitution_conv_zero] at h2
+            simp [clean_this_mess_asap] at h2
+            have h3 := substitution_type_eq (And.left ihppId) h2
+            simp [←lift_n_substitution] at h3
+            simp [n_substitution_zero] at h3
+            simp [zero_substitution] at h3
+            simp [clean_this_mess_too] at h3
+            apply h3
+            any_goals omega
+          · apply IsEqualType.type_trans
+            rotate_right
+            · apply B'⌈(ₛidₚ), a₂, a₄, p⌉
+            · rw [context_to_gen_ctx] at ihBB
+              rw [←middle_expand_context (Γ := Γ ⬝ A)] at ihBB
+              have h1 := (And.left (And.right substitution)
+                          (leq := Nat.le_step (Nat.le_step (Nat.le_refl n))))
+                          (And.right ihBB) (And.left (And.right ihaaA))
+              simp [substitute_into_gen_ctx] at h1
+              rw [n_substitution_zero] at h1
+              rw [zero_substitution] at h1
+              rw [substitution_conv_zero] at h1
+              rw [substitution_shift_substitute_zero] at h1
+              rw [middle_expand_context] at h1
+              have h2 := (And.left (And.right functionality_typing))
+                          (IsEqualTerm.ty_conv_eq (IsEqualTerm.term_symm haaA') (IsEqualType.type_symm hAA))
+                          (HasType.ty_conv (And.left (And.right ihaaA')) (IsEqualType.type_symm hAA))
+                          (HasType.ty_conv (And.left ihaaA') (IsEqualType.type_symm hAA)) 
+                          h1
+              simp [substitute_into_gen_ctx] at h2
+              simp [expand_ctx] at h2
+              rw [←lift_n_substitution] at h2
+              simp [n_substitution_zero] at h2
+              simp [zero_substitution] at h2
+              simp [substitution_conv_zero] at h2
+              simp [clean_this_mess_asap] at h2
+              have hnew : Γ ⊢ a₁ ≃[A] a₃ ≡ a₂ ≃[A] a₄ type :=
+                  IsEqualType.iden_form_eq (defeq_refl_type (And.left ihAA))
+                      haaA (IsEqualTerm.ty_conv_eq haaA' (IsEqualType.type_symm hAA))
+              have h3 := substitution_type_eq (HasType.ty_conv (And.left ihppId) hnew) h2
+              simp [←lift_n_substitution] at h3
+              simp [n_substitution_zero] at h3
+              simp [zero_substitution] at h3
+              simp [clean_this_mess_too] at h3
+              apply (IsEqualType.type_symm h3)
+              any_goals omega
+            · rw [context_to_gen_ctx] at ihBB
+              rw [←middle_expand_context (Γ := Γ ⬝ A)] at ihBB
+              have h1 := (And.left (And.right substitution)
+                          (leq := Nat.le_step (Nat.le_step (Nat.le_refl n))))
+                          (And.right ihBB) (And.left (And.right ihaaA))
+              simp [substitute_into_gen_ctx] at h1
+              rw [n_substitution_zero] at h1
+              rw [zero_substitution] at h1
+              rw [substitution_conv_zero] at h1
+              rw [substitution_shift_substitute_zero] at h1
+              rw [middle_expand_context] at h1
+              have h2 := (And.left (And.right substitution)
+                          (leq := (Nat.le_step (Nat.le_refl n))))
+                          (h1) (HasType.ty_conv (And.left (And.right ihaaA')) (IsEqualType.type_symm hAA))
+              simp [substitute_into_gen_ctx] at h2
+              simp [expand_ctx] at h2
+              rw [←lift_n_substitution] at h2
+              simp [n_substitution_zero] at h2
+              simp [zero_substitution] at h2
+              simp [substitution_conv_zero] at h2
+              simp [clean_this_mess_asap] at h2
+              have hlol := ctx_extr (boundary_ctx_type h2)
+              have hnew : Γ ⊢ a₁ ≃[A] a₃ ≡ a₂ ≃[A] a₄ type :=
+                  IsEqualType.iden_form_eq (defeq_refl_type (And.left ihAA))
+                      haaA (IsEqualTerm.ty_conv_eq haaA' (IsEqualType.type_symm hAA))
+              have hnew_old := context_conversion_type
+                                (And.right (And.right ihppId)) (IsEqualType.type_symm hnew) h2
+              have h3 := functionality_typing_type
+                          hnew_old
+                          (IsEqualTerm.term_symm hppId)
+                          (And.left (And.right ihppId))
+                          (And.left ihppId)
+              simp [←lift_n_substitution] at h3
+              simp [n_substitution_zero] at h3
+              simp [zero_substitution] at h3
+              simp [clean_this_mess_too] at h3
+              apply (IsEqualType.type_symm h3)
+              any_goals omega
+    · rw [context_to_gen_ctx] at ihBB
+      rw [←middle_expand_context (Γ := Γ ⬝ A)] at ihBB
+      have h := And.left (And.right substitution) (leq := Nat.le_step (Nat.le_step (Nat.le_refl n))) 
+                  (And.left ihBB) (And.left ihaaA)
+      simp [substitute_into_gen_ctx] at h
+      rw [n_substitution_zero] at h
+      rw [zero_substitution] at h
+      rw [substitution_conv_zero] at h
+      rw [substitution_shift_substitute_zero] at h
+      rw [middle_expand_context] at h
+      have h2 := And.left (And.right substitution) (leq := Nat.le_step (Nat.le_refl n)) 
+                  h (HasType.ty_conv (And.left ihaaA') (IsEqualType.type_symm hAA))
+      simp [substitute_into_gen_ctx] at h2
+      simp [expand_ctx] at h2
+      rw [←lift_n_substitution] at h2
+      simp [n_substitution_zero] at h2
+      simp [zero_substitution] at h2
+      simp [substitution_conv_zero] at h2
+      simp [clean_this_mess_asap] at h2
+      have h3 := substitution_type (And.left ihppId) h2
+      simp [←lift_n_substitution] at h3
+      simp [n_substitution_zero] at h3
+      simp [zero_substitution] at h3
+      rw [clean_this_mess_too] at h3
+      apply h3
+      any_goals omega
 
-theorem boundary_univ_unit_eq :
-    ∀ {n : Nat} {Γ : Ctx n}, Γ ctx → Γ ctx → (Γ ⊢ 𝟙 ∶ 𝒰) ∧ (Γ ⊢ 𝟙 ∶ 𝒰) ∧ Γ ⊢ 𝒰 type :=
-  by
-    intro n Γ hiC ihiC
-    repeat' apply And.intro
-    · apply HasType.univ_unit hiC
-    · apply HasType.univ_unit hiC
-    · apply IsType.univ_form hiC
-
-theorem boundary_univ_empty_eq :
-    ∀ {n : Nat} {Γ : Ctx n}, Γ ctx → Γ ctx → (Γ ⊢ 𝟘 ∶ 𝒰) ∧ (Γ ⊢ 𝟘 ∶ 𝒰) ∧ Γ ⊢ 𝒰 type :=
-  by
-    intro n Γ hiC ihiC
-    repeat' apply And.intro
-    · apply HasType.univ_empty hiC
-    · apply HasType.univ_empty hiC
-    · apply IsType.univ_form hiC
-
-theorem boundary_univ_pi_eq :
-    ∀ {n : Nat} {Γ : Ctx n} {A A' : Tm n} {B B' : Tm (n + 1)},
-    (Γ ⊢ A ≡ A' ∶ 𝒰) →
-    (Γ ⬝ A ⊢ B ≡ B' ∶ 𝒰) →
-    (Γ ⊢ A ∶ 𝒰) ∧ (Γ ⊢ A' ∶ 𝒰) ∧ Γ ⊢ 𝒰 type →
-    (Γ ⬝ A ⊢ B ∶ 𝒰) ∧ (Γ ⬝ A ⊢ B' ∶ 𝒰) ∧ Γ ⬝ A ⊢ 𝒰 type → (Γ ⊢ ΠA;B ∶ 𝒰) ∧ (Γ ⊢ ΠA';B' ∶ 𝒰) ∧ Γ ⊢ 𝒰 type :=
-  by
-    intro n Γ A A' B B' hAAU hBBU ihAAU ihBBU
-    repeat' apply And.intro
-    · apply HasType.univ_pi
-      · apply And.left ihAAU
-      · apply And.left ihBBU
-    · apply HasType.univ_pi
-      · apply And.left (And.right ihAAU)
-      · apply context_conversion_term
-        · apply IsType.univ_elim (And.left (And.right ihAAU))
-        · apply IsEqualType.univ_elim_eq hAAU
-        · apply And.left (And.right ihBBU)
-    · apply IsType.univ_form (boundary_ctx_term_eq hAAU)
-
-
-theorem boundary_univ_sigma_eq :
-    ∀ {n : Nat} {Γ : Ctx n} {A A' : Tm n} {B B' : Tm (n + 1)},
-    (Γ ⊢ A ≡ A' ∶ 𝒰) →
-      (Γ ⬝ A ⊢ B ≡ B' ∶ 𝒰) →
-        (Γ ⊢ A ∶ 𝒰) ∧ (Γ ⊢ A' ∶ 𝒰) ∧ Γ ⊢ 𝒰 type →
-          (Γ ⬝ A ⊢ B ∶ 𝒰) ∧ (Γ ⬝ A ⊢ B' ∶ 𝒰) ∧ Γ ⬝ A ⊢ 𝒰 type → (Γ ⊢ ΣA;B ∶ 𝒰) ∧ (Γ ⊢ ΣA';B' ∶ 𝒰) ∧ Γ ⊢ 𝒰 type :=
-  by
-    intro n Γ A A' B B' hAAU hBBU ihAAU ihBBU
-    repeat' apply And.intro
-    · apply HasType.univ_sigma
-      · apply And.left ihAAU
-      · apply And.left ihBBU
-    · apply HasType.univ_sigma
-      · apply And.left (And.right ihAAU)
-      · apply context_conversion_term
-        · apply IsType.univ_elim (And.left (And.right ihAAU))
-        · apply IsEqualType.univ_elim_eq hAAU
-        · apply And.left (And.right ihBBU)
-    · apply IsType.univ_form (boundary_ctx_term_eq hAAU)
-
-theorem boundary_univ_iden_eq :
-    ∀ {n : Nat} {Γ : Ctx n} {A A' a₁ a₂ a₃ a₄ : Tm n},
-    (Γ ⊢ A ≡ A' ∶ 𝒰) →
-      (Γ ⊢ a₁ ≡ a₂ ∶ A) →
-        (Γ ⊢ a₃ ≡ a₄ ∶ A) →
-          (Γ ⊢ A ∶ 𝒰) ∧ (Γ ⊢ A' ∶ 𝒰) ∧ Γ ⊢ 𝒰 type →
-            (Γ ⊢ a₁ ∶ A) ∧ (Γ ⊢ a₂ ∶ A) ∧ Γ ⊢ A type →
-              (Γ ⊢ a₃ ∶ A) ∧ (Γ ⊢ a₄ ∶ A) ∧ Γ ⊢ A type → (Γ ⊢ a₁ ≃[A] a₃ ∶ 𝒰) ∧ (Γ ⊢ a₂ ≃[A'] a₄ ∶ 𝒰) ∧ Γ ⊢ 𝒰 type :=
-  by
-    intro n Γ A A' a₁ a₂ a₃ a₄ hAAU haaA haaA' ihAAU ihaaA ihaaA'
-    repeat' apply And.intro
-    · apply HasType.univ_iden
-      · apply And.left ihAAU
-      · apply And.left ihaaA
-      · apply And.left ihaaA'
-    · apply HasType.univ_iden
-      · apply And.left (And.right ihAAU)
-      · apply HasType.ty_conv
-        · apply And.left (And.right ihaaA)
-        · apply IsEqualType.univ_elim_eq hAAU
-      · apply HasType.ty_conv
-        · apply And.left (And.right ihaaA')
-        · apply IsEqualType.univ_elim_eq hAAU
-    · apply And.right (And.right ihAAU)
-
-theorem boundary_ty_conv_eq :
-    ∀ {n : Nat} {Γ : Ctx n} {a b A B : Tm n},
-    (Γ ⊢ a ≡ b ∶ A) →
-      Γ ⊢ A ≡ B type →
-        (Γ ⊢ a ∶ A) ∧ (Γ ⊢ b ∶ A) ∧ Γ ⊢ A type → Γ ⊢ A type ∧ Γ ⊢ B type → (Γ ⊢ a ∶ B) ∧ (Γ ⊢ b ∶ B) ∧ Γ ⊢ B type :=
-  by
-    intro n Γ a b A B habA hAB ihabA ihAB
-    repeat' apply And.intro
-    · apply HasType.ty_conv
-      · apply And.left ihabA
-      · apply hAB
-    · apply HasType.ty_conv
-      · apply And.left (And.right ihabA)
-      · apply hAB
-    · apply And.right ihAB
-
-theorem boundary_term_symm :
-    ∀ {n : Nat} {Γ : Ctx n} {a a' A : Tm n},
-    (Γ ⊢ a ≡ a' ∶ A) → (Γ ⊢ a ∶ A) ∧ (Γ ⊢ a' ∶ A) ∧ Γ ⊢ A type → (Γ ⊢ a' ∶ A) ∧ (Γ ⊢ a ∶ A) ∧ Γ ⊢ A type :=
-  by
-    intro n Γ a a' A haaA ihaaA
-    repeat' apply And.intro
-    · apply And.left (And.right ihaaA)
-    · apply And.left ihaaA
-    · apply And.right (And.right ihaaA)
-
-theorem boundary_term_trans :
-    ∀ {n : Nat} {Γ : Ctx n} {T a b c : Tm n},
-    (Γ ⊢ a ≡ b ∶ T) →
-      (Γ ⊢ b ≡ c ∶ T) →
-        (Γ ⊢ a ∶ T) ∧ (Γ ⊢ b ∶ T) ∧ Γ ⊢ T type →
-          (Γ ⊢ b ∶ T) ∧ (Γ ⊢ c ∶ T) ∧ Γ ⊢ T type → (Γ ⊢ a ∶ T) ∧ (Γ ⊢ c ∶ T) ∧ Γ ⊢ T type :=
-  by
-    intro n Γ T a b c habT hbcT ihabT ihbcT
-    repeat' apply And.intro
-    · apply And.left ihabT
-    · apply And.left (And.right ihbcT)
-    · apply And.right (And.right ihabT)
+-- theorem boundary_univ_unit_eq :
+--     ∀ {n : Nat} {Γ : Ctx n}, Γ ctx → Γ ctx → (Γ ⊢ 𝟙 ∶ 𝒰) ∧ (Γ ⊢ 𝟙 ∶ 𝒰) ∧ Γ ⊢ 𝒰 type :=
+--   by
+--     intro n Γ hiC ihiC
+--     repeat' apply And.intro
+--     · apply HasType.univ_unit hiC
+--     · apply HasType.univ_unit hiC
+--     · apply IsType.univ_form hiC
+-- 
+-- theorem boundary_univ_empty_eq :
+--     ∀ {n : Nat} {Γ : Ctx n}, Γ ctx → Γ ctx → (Γ ⊢ 𝟘 ∶ 𝒰) ∧ (Γ ⊢ 𝟘 ∶ 𝒰) ∧ Γ ⊢ 𝒰 type :=
+--   by
+--     intro n Γ hiC ihiC
+--     repeat' apply And.intro
+--     · apply HasType.univ_empty hiC
+--     · apply HasType.univ_empty hiC
+--     · apply IsType.univ_form hiC
+-- 
+-- theorem boundary_univ_pi_eq :
+--     ∀ {n : Nat} {Γ : Ctx n} {A A' : Tm n} {B B' : Tm (n + 1)},
+--     (Γ ⊢ A ≡ A' ∶ 𝒰) →
+--     (Γ ⬝ A ⊢ B ≡ B' ∶ 𝒰) →
+--     (Γ ⊢ A ∶ 𝒰) ∧ (Γ ⊢ A' ∶ 𝒰) ∧ Γ ⊢ 𝒰 type →
+--     (Γ ⬝ A ⊢ B ∶ 𝒰) ∧ (Γ ⬝ A ⊢ B' ∶ 𝒰) ∧ Γ ⬝ A ⊢ 𝒰 type → (Γ ⊢ ΠA;B ∶ 𝒰) ∧ (Γ ⊢ ΠA';B' ∶ 𝒰) ∧ Γ ⊢ 𝒰 type :=
+--   by
+--     intro n Γ A A' B B' hAAU hBBU ihAAU ihBBU
+--     repeat' apply And.intro
+--     · apply HasType.univ_pi
+--       · apply And.left ihAAU
+--       · apply And.left ihBBU
+--     · apply HasType.univ_pi
+--       · apply And.left (And.right ihAAU)
+--       · apply context_conversion_term
+--         · apply IsType.univ_elim (And.left (And.right ihAAU))
+--         · apply IsEqualType.univ_elim_eq hAAU
+--         · apply And.left (And.right ihBBU)
+--     · apply IsType.univ_form (boundary_ctx_term_eq hAAU)
+-- 
+-- 
+-- theorem boundary_univ_sigma_eq :
+--     ∀ {n : Nat} {Γ : Ctx n} {A A' : Tm n} {B B' : Tm (n + 1)},
+--     (Γ ⊢ A ≡ A' ∶ 𝒰) →
+--       (Γ ⬝ A ⊢ B ≡ B' ∶ 𝒰) →
+--         (Γ ⊢ A ∶ 𝒰) ∧ (Γ ⊢ A' ∶ 𝒰) ∧ Γ ⊢ 𝒰 type →
+--           (Γ ⬝ A ⊢ B ∶ 𝒰) ∧ (Γ ⬝ A ⊢ B' ∶ 𝒰) ∧ Γ ⬝ A ⊢ 𝒰 type → (Γ ⊢ ΣA;B ∶ 𝒰) ∧ (Γ ⊢ ΣA';B' ∶ 𝒰) ∧ Γ ⊢ 𝒰 type :=
+--   by
+--     intro n Γ A A' B B' hAAU hBBU ihAAU ihBBU
+--     repeat' apply And.intro
+--     · apply HasType.univ_sigma
+--       · apply And.left ihAAU
+--       · apply And.left ihBBU
+--     · apply HasType.univ_sigma
+--       · apply And.left (And.right ihAAU)
+--       · apply context_conversion_term
+--         · apply IsType.univ_elim (And.left (And.right ihAAU))
+--         · apply IsEqualType.univ_elim_eq hAAU
+--         · apply And.left (And.right ihBBU)
+--     · apply IsType.univ_form (boundary_ctx_term_eq hAAU)
+-- 
+-- theorem boundary_univ_nat_eq :
+--     ∀ {n : Nat} {Γ : Ctx n}, Γ ctx → Γ ctx → (Γ ⊢ 𝒩 ∶ 𝒰) ∧ (Γ ⊢ 𝒩 ∶ 𝒰) ∧ Γ ⊢ 𝒰 type :=
+--   by
+--     intro n Γ hiC ihiC
+--     repeat' apply And.intro
+--     · apply HasType.univ_nat hiC
+--     · apply HasType.univ_nat hiC
+--     · apply IsType.univ_form hiC
+-- 
+-- theorem boundary_univ_iden_eq :
+--     ∀ {n : Nat} {Γ : Ctx n} {A A' a₁ a₂ a₃ a₄ : Tm n},
+--     (Γ ⊢ A ≡ A' ∶ 𝒰) →
+--       (Γ ⊢ a₁ ≡ a₂ ∶ A) →
+--         (Γ ⊢ a₃ ≡ a₄ ∶ A) →
+--           (Γ ⊢ A ∶ 𝒰) ∧ (Γ ⊢ A' ∶ 𝒰) ∧ Γ ⊢ 𝒰 type →
+--             (Γ ⊢ a₁ ∶ A) ∧ (Γ ⊢ a₂ ∶ A) ∧ Γ ⊢ A type →
+--               (Γ ⊢ a₃ ∶ A) ∧ (Γ ⊢ a₄ ∶ A) ∧ Γ ⊢ A type → (Γ ⊢ a₁ ≃[A] a₃ ∶ 𝒰) ∧ (Γ ⊢ a₂ ≃[A'] a₄ ∶ 𝒰) ∧ Γ ⊢ 𝒰 type :=
+--   by
+--     intro n Γ A A' a₁ a₂ a₃ a₄ hAAU haaA haaA' ihAAU ihaaA ihaaA'
+--     repeat' apply And.intro
+--     · apply HasType.univ_iden
+--       · apply And.left ihAAU
+--       · apply And.left ihaaA
+--       · apply And.left ihaaA'
+--     · apply HasType.univ_iden
+--       · apply And.left (And.right ihAAU)
+--       · apply HasType.ty_conv
+--         · apply And.left (And.right ihaaA)
+--         · apply IsEqualType.univ_elim_eq hAAU
+--       · apply HasType.ty_conv
+--         · apply And.left (And.right ihaaA')
+--         · apply IsEqualType.univ_elim_eq hAAU
+--     · apply And.right (And.right ihAAU)
+-- 
+-- theorem boundary_ty_conv_eq :
+--     ∀ {n : Nat} {Γ : Ctx n} {a b A B : Tm n},
+--     (Γ ⊢ a ≡ b ∶ A) →
+--       Γ ⊢ A ≡ B type →
+--         (Γ ⊢ a ∶ A) ∧ (Γ ⊢ b ∶ A) ∧ Γ ⊢ A type → Γ ⊢ A type ∧ Γ ⊢ B type → (Γ ⊢ a ∶ B) ∧ (Γ ⊢ b ∶ B) ∧ Γ ⊢ B type :=
+--   by
+--     intro n Γ a b A B habA hAB ihabA ihAB
+--     repeat' apply And.intro
+--     · apply HasType.ty_conv
+--       · apply And.left ihabA
+--       · apply hAB
+--     · apply HasType.ty_conv
+--       · apply And.left (And.right ihabA)
+--       · apply hAB
+--     · apply And.right ihAB
+-- 
+-- theorem boundary_term_symm :
+--     ∀ {n : Nat} {Γ : Ctx n} {a a' A : Tm n},
+--     (Γ ⊢ a ≡ a' ∶ A) → (Γ ⊢ a ∶ A) ∧ (Γ ⊢ a' ∶ A) ∧ Γ ⊢ A type → (Γ ⊢ a' ∶ A) ∧ (Γ ⊢ a ∶ A) ∧ Γ ⊢ A type :=
+--   by
+--     intro n Γ a a' A haaA ihaaA
+--     repeat' apply And.intro
+--     · apply And.left (And.right ihaaA)
+--     · apply And.left ihaaA
+--     · apply And.right (And.right ihaaA)
+-- 
+-- theorem boundary_term_trans :
+--     ∀ {n : Nat} {Γ : Ctx n} {T a b c : Tm n},
+--     (Γ ⊢ a ≡ b ∶ T) →
+--       (Γ ⊢ b ≡ c ∶ T) →
+--         (Γ ⊢ a ∶ T) ∧ (Γ ⊢ b ∶ T) ∧ Γ ⊢ T type →
+--           (Γ ⊢ b ∶ T) ∧ (Γ ⊢ c ∶ T) ∧ Γ ⊢ T type → (Γ ⊢ a ∶ T) ∧ (Γ ⊢ c ∶ T) ∧ Γ ⊢ T type :=
+--   by
+--     intro n Γ T a b c habT hbcT ihabT ihbcT
+--     repeat' apply And.intro
+--     · apply And.left ihabT
+--     · apply And.left (And.right ihbcT)
+--     · apply And.right (And.right ihabT)
