IMLTT/untyped/proofs/Conversion.lean
@@ -207,8 +207,10 @@ theorem conversion_var_substitute {σ σ' : Subst m n} :
             apply ξ
           · apply conversion_var_lift_n h
         · apply And.intro
-          · apply conversion_var_substitute h
-            assumption
+          · apply conversion_var_substitute
+            · have ξ := lift_subst_n 1 σ
+              apply ξ
+            · apply conversion_var_lift_n h
           · apply And.intro
             · apply conversion_var_substitute h
               assumption
@@ -358,7 +360,10 @@ theorem conversion_sub_weak :
           · apply conversion_var_lift_n
             apply conversion_var_sub_weak
         · apply And.intro
-          · apply conversion_sub_weak
+          · apply conversion_var_substitute
+            · apply lift_subst_n 1 (.weak ρ)
+            · apply conversion_var_lift_n
+              apply conversion_var_sub_weak
           · apply And.intro
             · apply conversion_sub_weak
             · apply And.intro
